<?xml version="1.0"?>
<rdf:RDF xmlns="https://raw.githubusercontent.com/ranacoskun/cognitive_bias_ontology/main/misattributionOfMemory.owl"
     xml:base="https://raw.githubusercontent.com/ranacoskun/cognitive_bias_ontology/main/misattributionOfMemory.owl"
     xmlns:dc="http://purl.org/dc/elements/1.1/"
     xmlns:cbi="https://raw.githubusercontent.com/ranacoskun/cognitive_bias_ontology/main/cbi.owl"
     xmlns:mom="https://raw.githubusercontent.com/ranacoskun/cognitive_bias_ontology/main/misattributionOfMemory.owl"
     xmlns:owl="http://www.w3.org/2002/07/owl#"
     xmlns:rdf="http://www.w3.org/1999/02/22-rdf-syntax-ns#"
     xmlns:xml="http://www.w3.org/XML/1998/namespace"
     xmlns:xsd="http://www.w3.org/2001/XMLSchema#"
     xmlns:rdfs="http://www.w3.org/2000/01/rdf-schema#">
    <owl:Ontology rdf:about="https://raw.githubusercontent.com/ranacoskun/cognitive_bias_ontology/main/misattributionOfMemory.owl">
        <dc:creator>Francesco Alaimo</dc:creator>
        <dc:title>Misattribution of memory</dc:title>
        <rdfs:comment>This is an ontology that describes the behaviour of a person affected by the Misattribution of memory bias.</rdfs:comment>
    </owl:Ontology>
    


    <!-- 
    ///////////////////////////////////////////////////////////////////////////////////////
    //
    // Annotation properties
    //
    ///////////////////////////////////////////////////////////////////////////////////////
     -->

    


    <!-- http://purl.org/dc/elements/1.1/creator -->

    <owl:AnnotationProperty rdf:about="http://purl.org/dc/elements/1.1/creator"/>
    


    <!-- http://purl.org/dc/elements/1.1/title -->

    <owl:AnnotationProperty rdf:about="http://purl.org/dc/elements/1.1/title"/>
    


    <!-- http://www.w3.org/2000/01/rdf-schema#label -->

    <owl:AnnotationProperty rdf:about="http://www.w3.org/2000/01/rdf-schema#label"/>
    


    <!-- 
    ///////////////////////////////////////////////////////////////////////////////////////
    //
    // Object Properties
    //
    ///////////////////////////////////////////////////////////////////////////////////////
     -->

    


    <!-- https://raw.githubusercontent.com/ranacoskun/cognitive_bias_ontology/main/misattributionOfMemory.owl#affects -->

    <owl:ObjectProperty rdf:about="https://raw.githubusercontent.com/ranacoskun/cognitive_bias_ontology/main/misattributionOfMemory.owl#affects">
        <rdfs:subPropertyOf rdf:resource="http://www.w3.org/2002/07/owl#topObjectProperty"/>
        <owl:inverseOf rdf:resource="https://raw.githubusercontent.com/ranacoskun/cognitive_bias_ontology/main/misattributionOfMemory.owl#isAffectedBy"/>
        <rdfs:domain rdf:resource="https://raw.githubusercontent.com/ranacoskun/cognitive_bias_ontology/main/cbi.owl#Cryptomnesia"/>
        <rdfs:domain rdf:resource="https://raw.githubusercontent.com/ranacoskun/cognitive_bias_ontology/main/cbi.owl#FalseMemory"/>
        <rdfs:domain rdf:resource="https://raw.githubusercontent.com/ranacoskun/cognitive_bias_ontology/main/cbi.owl#SourceConfusion"/>
        <rdfs:range rdf:resource="https://raw.githubusercontent.com/ranacoskun/cognitive_bias_ontology/main/cbi.owl#BiasedAgent"/>
    </owl:ObjectProperty>
    


    <!-- https://raw.githubusercontent.com/ranacoskun/cognitive_bias_ontology/main/misattributionOfMemory.owl#canBeCorrectedBy -->

    <owl:ObjectProperty rdf:about="https://raw.githubusercontent.com/ranacoskun/cognitive_bias_ontology/main/misattributionOfMemory.owl#canBeCorrectedBy">
        <rdfs:domain rdf:resource="https://raw.githubusercontent.com/ranacoskun/cognitive_bias_ontology/main/cbi.owl#FalseMemory"/>
        <rdfs:range rdf:resource="https://raw.githubusercontent.com/ranacoskun/cognitive_bias_ontology/main/misattributionOfMemory.owl#Correction"/>
        <rdfs:comment>Describes the relation between the bias and the correction to enact</rdfs:comment>
    </owl:ObjectProperty>
    


    <!-- https://raw.githubusercontent.com/ranacoskun/cognitive_bias_ontology/main/misattributionOfMemory.owl#canBePreventedBy -->

    <owl:ObjectProperty rdf:about="https://raw.githubusercontent.com/ranacoskun/cognitive_bias_ontology/main/misattributionOfMemory.owl#canBePreventedBy">
        <rdfs:domain rdf:resource="https://raw.githubusercontent.com/ranacoskun/cognitive_bias_ontology/main/cbi.owl#FalseMemory"/>
        <rdfs:range rdf:resource="https://raw.githubusercontent.com/ranacoskun/cognitive_bias_ontology/main/misattributionOfMemory.owl#Prevention"/>
        <rdfs:comment>Describes the relation between the bias and the prevention techniques to it</rdfs:comment>
    </owl:ObjectProperty>
    


    <!-- https://raw.githubusercontent.com/ranacoskun/cognitive_bias_ontology/main/misattributionOfMemory.owl#creates -->

    <owl:ObjectProperty rdf:about="https://raw.githubusercontent.com/ranacoskun/cognitive_bias_ontology/main/misattributionOfMemory.owl#creates">
        <rdfs:domain rdf:resource="http://etna.istc.cnr.it/framester2/data/framestercore/People"/>
        <rdfs:range rdf:resource="https://raw.githubusercontent.com/ranacoskun/cognitive_bias_ontology/main/misattributionOfMemory.owl#RecalledIdea"/>
        <rdfs:comment>Creates the relation between the person affected by the bias and the creation of a self assessed original creation</rdfs:comment>
    </owl:ObjectProperty>
    


    <!-- https://raw.githubusercontent.com/ranacoskun/cognitive_bias_ontology/main/misattributionOfMemory.owl#forgets -->

    <owl:ObjectProperty rdf:about="https://raw.githubusercontent.com/ranacoskun/cognitive_bias_ontology/main/misattributionOfMemory.owl#forgets">
        <rdfs:domain rdf:resource="http://etna.istc.cnr.it/framester2/data/framestercore/People"/>
        <rdfs:range rdf:resource="https://raw.githubusercontent.com/ranacoskun/cognitive_bias_ontology/main/misattributionOfMemory.owl#OriginalSource"/>
        <rdfs:comment>Describes the lost of memory from the biased agents towards the Original Source</rdfs:comment>
    </owl:ObjectProperty>
    


    <!-- https://raw.githubusercontent.com/ranacoskun/cognitive_bias_ontology/main/misattributionOfMemory.owl#generatedBy -->

    <owl:ObjectProperty rdf:about="https://raw.githubusercontent.com/ranacoskun/cognitive_bias_ontology/main/misattributionOfMemory.owl#generatedBy">
        <rdfs:domain>
            <owl:Class>
                <owl:unionOf rdf:parseType="Collection">
                    <rdf:Description rdf:about="http://etna.istc.cnr.it/framester2/data/framestercore/Memorization"/>
                    <rdf:Description rdf:about="https://raw.githubusercontent.com/ranacoskun/cognitive_bias_ontology/main/cbi.owl#SourceConfusion"/>
                </owl:unionOf>
            </owl:Class>
        </rdfs:domain>
        <rdfs:range rdf:resource="http://etna.istc.cnr.it/framester2/data/framestercore/Event"/>
        <rdfs:range rdf:resource="https://raw.githubusercontent.com/ranacoskun/cognitive_bias_ontology/main/misattributionOfMemory.owl#OriginalSource"/>
        <rdfs:comment>Describes the relation between a bias and the source from which it starts or come from</rdfs:comment>
    </owl:ObjectProperty>
    


    <!-- https://raw.githubusercontent.com/ranacoskun/cognitive_bias_ontology/main/misattributionOfMemory.owl#hasCause -->

    <owl:ObjectProperty rdf:about="https://raw.githubusercontent.com/ranacoskun/cognitive_bias_ontology/main/misattributionOfMemory.owl#hasCause">
        <rdfs:domain rdf:resource="https://raw.githubusercontent.com/ranacoskun/cognitive_bias_ontology/main/cbi.owl#FalseMemory"/>
        <rdfs:range rdf:resource="https://raw.githubusercontent.com/ranacoskun/cognitive_bias_ontology/main/misattributionOfMemory.owl#Cause"/>
        <rdfs:comment>Describes the relation between the a Bias and its inherent cause</rdfs:comment>
    </owl:ObjectProperty>
    


    <!-- https://raw.githubusercontent.com/ranacoskun/cognitive_bias_ontology/main/misattributionOfMemory.owl#hasEffect -->

    <owl:ObjectProperty rdf:about="https://raw.githubusercontent.com/ranacoskun/cognitive_bias_ontology/main/misattributionOfMemory.owl#hasEffect">
        <rdfs:domain rdf:resource="https://raw.githubusercontent.com/ranacoskun/cognitive_bias_ontology/main/cbi.owl#FalseMemory"/>
        <rdfs:range rdf:resource="https://raw.githubusercontent.com/ranacoskun/cognitive_bias_ontology/main/misattributionOfMemory.owl#Effect"/>
        <rdfs:comment>Describes the relation between the bias and its effect</rdfs:comment>
    </owl:ObjectProperty>
    


    <!-- https://raw.githubusercontent.com/ranacoskun/cognitive_bias_ontology/main/misattributionOfMemory.owl#hasParticipant -->

    <owl:ObjectProperty rdf:about="https://raw.githubusercontent.com/ranacoskun/cognitive_bias_ontology/main/misattributionOfMemory.owl#hasParticipant">
        <rdfs:domain rdf:resource="http://etna.istc.cnr.it/framester2/data/framestercore/Event"/>
        <rdfs:domain rdf:resource="https://raw.githubusercontent.com/ranacoskun/cognitive_bias_ontology/main/misattributionOfMemory.owl#CognitiveError"/>
        <rdfs:range rdf:resource="http://etna.istc.cnr.it/framester2/data/framestercore/People"/>
        <rdfs:comment>Describes the relation between the Event and the Biased Agent who participate</rdfs:comment>
    </owl:ObjectProperty>
    


    <!-- https://raw.githubusercontent.com/ranacoskun/cognitive_bias_ontology/main/misattributionOfMemory.owl#isAffectedBy -->

    <owl:ObjectProperty rdf:about="https://raw.githubusercontent.com/ranacoskun/cognitive_bias_ontology/main/misattributionOfMemory.owl#isAffectedBy">
        <rdfs:domain rdf:resource="https://raw.githubusercontent.com/ranacoskun/cognitive_bias_ontology/main/cbi.owl#BiasedAgent"/>
        <rdfs:range rdf:resource="https://raw.githubusercontent.com/ranacoskun/cognitive_bias_ontology/main/cbi.owl#Cryptomnesia"/>
        <rdfs:range rdf:resource="https://raw.githubusercontent.com/ranacoskun/cognitive_bias_ontology/main/cbi.owl#FalseMemory"/>
        <rdfs:range rdf:resource="https://raw.githubusercontent.com/ranacoskun/cognitive_bias_ontology/main/cbi.owl#SourceConfusion"/>
        <rdfs:comment>Describes the relationship between Biased Agent and Bias</rdfs:comment>
    </owl:ObjectProperty>
    


    <!-- https://raw.githubusercontent.com/ranacoskun/cognitive_bias_ontology/main/misattributionOfMemory.owl#isAssessedBy -->

    <owl:ObjectProperty rdf:about="https://raw.githubusercontent.com/ranacoskun/cognitive_bias_ontology/main/misattributionOfMemory.owl#isAssessedBy">
        <rdfs:domain rdf:resource="https://raw.githubusercontent.com/ranacoskun/cognitive_bias_ontology/main/cbi.owl#FalseMemory"/>
        <rdfs:range rdf:resource="https://raw.githubusercontent.com/ranacoskun/cognitive_bias_ontology/main/misattributionOfMemory.owl#MemoryTest"/>
        <rdfs:comment>Describes the relation between the bias and the Memory Test</rdfs:comment>
    </owl:ObjectProperty>
    


    <!-- https://raw.githubusercontent.com/ranacoskun/cognitive_bias_ontology/main/misattributionOfMemory.owl#isDerivedFrom -->

    <owl:ObjectProperty rdf:about="https://raw.githubusercontent.com/ranacoskun/cognitive_bias_ontology/main/misattributionOfMemory.owl#isDerivedFrom">
        <rdfs:domain rdf:resource="https://raw.githubusercontent.com/ranacoskun/cognitive_bias_ontology/main/misattributionOfMemory.owl#RecalledIdea"/>
        <rdfs:range rdf:resource="https://raw.githubusercontent.com/ranacoskun/cognitive_bias_ontology/main/misattributionOfMemory.owl#OriginalSource"/>
        <rdfs:comment>Puts in relation the self assessed original creation and the true original source of it</rdfs:comment>
    </owl:ObjectProperty>
    


    <!-- https://raw.githubusercontent.com/ranacoskun/cognitive_bias_ontology/main/misattributionOfMemory.owl#isRecalledIn -->

    <owl:ObjectProperty rdf:about="https://raw.githubusercontent.com/ranacoskun/cognitive_bias_ontology/main/misattributionOfMemory.owl#isRecalledIn">
        <rdfs:domain rdf:resource="https://raw.githubusercontent.com/ranacoskun/cognitive_bias_ontology/main/misattributionOfMemory.owl#OriginalSource"/>
        <rdfs:range rdf:resource="https://raw.githubusercontent.com/ranacoskun/cognitive_bias_ontology/main/cbi.owl#Cryptomnesia"/>
        <rdfs:comment>Describes the relation between the original source and the current Bias</rdfs:comment>
    </owl:ObjectProperty>
    


    <!-- https://raw.githubusercontent.com/ranacoskun/cognitive_bias_ontology/main/misattributionOfMemory.owl#isSupportedOrRefutedBy -->

    <owl:ObjectProperty rdf:about="https://raw.githubusercontent.com/ranacoskun/cognitive_bias_ontology/main/misattributionOfMemory.owl#isSupportedOrRefutedBy">
        <rdfs:domain rdf:resource="https://raw.githubusercontent.com/ranacoskun/cognitive_bias_ontology/main/cbi.owl#FalseMemory"/>
        <rdfs:range rdf:resource="https://raw.githubusercontent.com/ranacoskun/cognitive_bias_ontology/main/misattributionOfMemory.owl#Evidence"/>
        <rdfs:comment>Describes the relation between the False Memory and the Evidence</rdfs:comment>
    </owl:ObjectProperty>
    


    <!-- https://raw.githubusercontent.com/ranacoskun/cognitive_bias_ontology/main/misattributionOfMemory.owl#leadsTo -->

    <owl:ObjectProperty rdf:about="https://raw.githubusercontent.com/ranacoskun/cognitive_bias_ontology/main/misattributionOfMemory.owl#leadsTo">
        <rdfs:domain rdf:resource="https://raw.githubusercontent.com/ranacoskun/cognitive_bias_ontology/main/misattributionOfMemory.owl#CognitiveError"/>
        <rdfs:range rdf:resource="https://raw.githubusercontent.com/ranacoskun/cognitive_bias_ontology/main/cbi.owl#SourceConfusion"/>
        <rdfs:comment>Describes the relation between the cognitive error and the bias</rdfs:comment>
    </owl:ObjectProperty>
    


    <!-- https://raw.githubusercontent.com/ranacoskun/cognitive_bias_ontology/main/misattributionOfMemory.owl#occursIn -->

    <owl:ObjectProperty rdf:about="https://raw.githubusercontent.com/ranacoskun/cognitive_bias_ontology/main/misattributionOfMemory.owl#occursIn">
        <rdfs:domain rdf:resource="https://raw.githubusercontent.com/ranacoskun/cognitive_bias_ontology/main/cbi.owl#Cryptomnesia"/>
        <rdfs:range rdf:resource="https://dbpedia.org/ontology/Media"/>
        <rdfs:comment>Puts in relation the current Bias and the Media through which it can be exposed</rdfs:comment>
    </owl:ObjectProperty>
    


    <!-- https://raw.githubusercontent.com/ranacoskun/cognitive_bias_ontology/main/misattributionOfMemory.owl#relatesToEvent -->

    <owl:ObjectProperty rdf:about="https://raw.githubusercontent.com/ranacoskun/cognitive_bias_ontology/main/misattributionOfMemory.owl#relatesToEvent">
        <rdfs:domain rdf:resource="https://raw.githubusercontent.com/ranacoskun/cognitive_bias_ontology/main/misattributionOfMemory.owl#CognitiveError"/>
        <rdfs:range rdf:resource="http://etna.istc.cnr.it/framester2/data/framestercore/Event"/>
        <rdfs:comment>Describes the relation between the Cognitive Error committed and the Event in which it takes place</rdfs:comment>
    </owl:ObjectProperty>
    


    <!-- 
    ///////////////////////////////////////////////////////////////////////////////////////
    //
    // Classes
    //
    ///////////////////////////////////////////////////////////////////////////////////////
     -->

    


    <!-- http://etna.istc.cnr.it/framester2/data/framestercore/Event -->

    <owl:Class rdf:about="http://etna.istc.cnr.it/framester2/data/framestercore/Event"/>
    


    <!-- http://etna.istc.cnr.it/framester2/data/framestercore/Memorization -->

    <owl:Class rdf:about="http://etna.istc.cnr.it/framester2/data/framestercore/Memorization"/>
    


    <!-- http://etna.istc.cnr.it/framester2/data/framestercore/People -->

    <owl:Class rdf:about="http://etna.istc.cnr.it/framester2/data/framestercore/People"/>
    


    <!-- https://dbpedia.org/ontology/Media -->

    <owl:Class rdf:about="https://dbpedia.org/ontology/Media"/>
    


    <!-- https://raw.githubusercontent.com/ranacoskun/cognitive_bias_ontology/main/cbi.owl#BiasedAgent -->

    <owl:Class rdf:about="https://raw.githubusercontent.com/ranacoskun/cognitive_bias_ontology/main/cbi.owl#BiasedAgent">
        <rdfs:subClassOf rdf:resource="http://etna.istc.cnr.it/framester2/data/framestercore/People"/>
        <rdfs:comment>Represents an entity that experiences the bias.</rdfs:comment>
    </owl:Class>
    


    <!-- https://raw.githubusercontent.com/ranacoskun/cognitive_bias_ontology/main/cbi.owl#CognitiveBias -->

    <owl:Class rdf:about="https://raw.githubusercontent.com/ranacoskun/cognitive_bias_ontology/main/cbi.owl#CognitiveBias">
        <rdfs:comment>Represents the overarching concept of cognitive biases.</rdfs:comment>
    </owl:Class>
    


    <!-- https://raw.githubusercontent.com/ranacoskun/cognitive_bias_ontology/main/cbi.owl#Cryptomnesia -->

    <owl:Class rdf:about="https://raw.githubusercontent.com/ranacoskun/cognitive_bias_ontology/main/cbi.owl#Cryptomnesia">
        <rdfs:subClassOf rdf:resource="https://raw.githubusercontent.com/ranacoskun/cognitive_bias_ontology/main/cbi.owl#MisattributedMemory"/>
        <rdfs:comment>Describes the occurence of the Cryptomnesia bias</rdfs:comment>
    </owl:Class>
    


    <!-- https://raw.githubusercontent.com/ranacoskun/cognitive_bias_ontology/main/cbi.owl#FalseMemory -->

    <owl:Class rdf:about="https://raw.githubusercontent.com/ranacoskun/cognitive_bias_ontology/main/cbi.owl#FalseMemory">
        <rdfs:subClassOf rdf:resource="https://raw.githubusercontent.com/ranacoskun/cognitive_bias_ontology/main/cbi.owl#MisattributedMemory"/>
        <rdfs:comment>Describes the False Memory bias occurrence</rdfs:comment>
    </owl:Class>
    


    <!-- https://raw.githubusercontent.com/ranacoskun/cognitive_bias_ontology/main/cbi.owl#MisattributedMemory -->

    <owl:Class rdf:about="https://raw.githubusercontent.com/ranacoskun/cognitive_bias_ontology/main/cbi.owl#MisattributedMemory">
        <rdfs:subClassOf rdf:resource="https://raw.githubusercontent.com/ranacoskun/cognitive_bias_ontology/main/cbi.owl#CognitiveBias"/>
        <rdfs:comment>Describes a generic Misattribution of Memory</rdfs:comment>
    </owl:Class>
    


    <!-- https://raw.githubusercontent.com/ranacoskun/cognitive_bias_ontology/main/cbi.owl#SourceConfusion -->

    <owl:Class rdf:about="https://raw.githubusercontent.com/ranacoskun/cognitive_bias_ontology/main/cbi.owl#SourceConfusion">
        <rdfs:subClassOf rdf:resource="https://raw.githubusercontent.com/ranacoskun/cognitive_bias_ontology/main/cbi.owl#MisattributedMemory"/>
        <owl:disjointWith rdf:resource="https://raw.githubusercontent.com/ranacoskun/cognitive_bias_ontology/main/misattributionOfMemory.owl#OriginalSource"/>
        <rdfs:comment>Describes the Source Confusion bias occurrence</rdfs:comment>
    </owl:Class>
    


    <!-- https://raw.githubusercontent.com/ranacoskun/cognitive_bias_ontology/main/misattributionOfMemory.owl#Cause -->

    <owl:Class rdf:about="https://raw.githubusercontent.com/ranacoskun/cognitive_bias_ontology/main/misattributionOfMemory.owl#Cause">
        <rdfs:comment>Factors that contribute to the formation of false memories</rdfs:comment>
    </owl:Class>
    


    <!-- https://raw.githubusercontent.com/ranacoskun/cognitive_bias_ontology/main/misattributionOfMemory.owl#CognitiveError -->

    <owl:Class rdf:about="https://raw.githubusercontent.com/ranacoskun/cognitive_bias_ontology/main/misattributionOfMemory.owl#CognitiveError">
        <rdfs:comment>A Cognitive error that leads to the Source Confusion bias, occurred during memorization</rdfs:comment>
    </owl:Class>
    


    <!-- https://raw.githubusercontent.com/ranacoskun/cognitive_bias_ontology/main/misattributionOfMemory.owl#Correction -->

    <owl:Class rdf:about="https://raw.githubusercontent.com/ranacoskun/cognitive_bias_ontology/main/misattributionOfMemory.owl#Correction">
        <rdfs:comment>Methods used to identify and correct false memories.</rdfs:comment>
    </owl:Class>
    


    <!-- https://raw.githubusercontent.com/ranacoskun/cognitive_bias_ontology/main/misattributionOfMemory.owl#Effect -->

    <owl:Class rdf:about="https://raw.githubusercontent.com/ranacoskun/cognitive_bias_ontology/main/misattributionOfMemory.owl#Effect">
        <rdfs:comment>The impact or consequences of false memories on individuals and society.</rdfs:comment>
    </owl:Class>
    


    <!-- https://raw.githubusercontent.com/ranacoskun/cognitive_bias_ontology/main/misattributionOfMemory.owl#Evidence -->

    <owl:Class rdf:about="https://raw.githubusercontent.com/ranacoskun/cognitive_bias_ontology/main/misattributionOfMemory.owl#Evidence">
        <rdfs:comment>Information or data used to support or refute the accuracy of a memory.</rdfs:comment>
    </owl:Class>
    


    <!-- https://raw.githubusercontent.com/ranacoskun/cognitive_bias_ontology/main/misattributionOfMemory.owl#MemoryTest -->

    <owl:Class rdf:about="https://raw.githubusercontent.com/ranacoskun/cognitive_bias_ontology/main/misattributionOfMemory.owl#MemoryTest">
        <rdfs:comment>Tools or techniques used to assess the accuracy of memories and identify false ones</rdfs:comment>
    </owl:Class>
    


    <!-- https://raw.githubusercontent.com/ranacoskun/cognitive_bias_ontology/main/misattributionOfMemory.owl#OriginalSource -->

    <owl:Class rdf:about="https://raw.githubusercontent.com/ranacoskun/cognitive_bias_ontology/main/misattributionOfMemory.owl#OriginalSource">
        <rdfs:comment>Describes the Original Source that causes the true instantiation of a memory</rdfs:comment>
    </owl:Class>
    


    <!-- https://raw.githubusercontent.com/ranacoskun/cognitive_bias_ontology/main/misattributionOfMemory.owl#Prevention -->

    <owl:Class rdf:about="https://raw.githubusercontent.com/ranacoskun/cognitive_bias_ontology/main/misattributionOfMemory.owl#Prevention">
        <rdfs:comment>Strategies or practices aimed at reducing the occurrence of false memories</rdfs:comment>
    </owl:Class>
    


    <!-- https://raw.githubusercontent.com/ranacoskun/cognitive_bias_ontology/main/misattributionOfMemory.owl#RecalledIdea -->

    <owl:Class rdf:about="https://raw.githubusercontent.com/ranacoskun/cognitive_bias_ontology/main/misattributionOfMemory.owl#RecalledIdea">
        <rdfs:comment>Describes the idea the biased agent thinks they&apos;ve just created, in this domain refers to a self assessed original creation of any kind, usually a sentence, a joke, a verse.</rdfs:comment>
    </owl:Class>
    


    <!-- 
    ///////////////////////////////////////////////////////////////////////////////////////
    //
    // Individuals
    //
    ///////////////////////////////////////////////////////////////////////////////////////
     -->

    


    <!-- https://raw.githubusercontent.com/ranacoskun/cognitive_bias_ontology/main/misattributionOfMemory.owl#CCTV_footage -->

    <owl:NamedIndividual rdf:about="https://raw.githubusercontent.com/ranacoskun/cognitive_bias_ontology/main/misattributionOfMemory.owl#CCTV_footage">
        <rdf:type rdf:resource="https://raw.githubusercontent.com/ranacoskun/cognitive_bias_ontology/main/misattributionOfMemory.owl#Evidence"/>
        <rdfs:comment>CCTV footage recorded from the bank where the robbery took place.</rdfs:comment>
    </owl:NamedIndividual>
    


    <!-- https://raw.githubusercontent.com/ranacoskun/cognitive_bias_ontology/main/misattributionOfMemory.owl#Jane_Doe -->

    <owl:NamedIndividual rdf:about="https://raw.githubusercontent.com/ranacoskun/cognitive_bias_ontology/main/misattributionOfMemory.owl#Jane_Doe">
        <rdf:type rdf:resource="https://raw.githubusercontent.com/ranacoskun/cognitive_bias_ontology/main/cbi.owl#BiasedAgent"/>
        <rdfs:comment>A passerby, Jane Doe, claimed to have seen the perpetrator flee the scene.</rdfs:comment>
    </owl:NamedIndividual>
    


    <!-- https://raw.githubusercontent.com/ranacoskun/cognitive_bias_ontology/main/misattributionOfMemory.owl#News_information -->

    <owl:NamedIndividual rdf:about="https://raw.githubusercontent.com/ranacoskun/cognitive_bias_ontology/main/misattributionOfMemory.owl#News_information">
        <rdf:type rdf:resource="https://raw.githubusercontent.com/ranacoskun/cognitive_bias_ontology/main/cbi.owl#SourceConfusion"/>
        <rdfs:comment>Remembering a news and thinking it was from an authorative source like a newspaper while it was seen in social medias</rdfs:comment>
    </owl:NamedIndividual>
    


    <!-- https://raw.githubusercontent.com/ranacoskun/cognitive_bias_ontology/main/misattributionOfMemory.owl#Social_Media -->

    <owl:NamedIndividual rdf:about="https://raw.githubusercontent.com/ranacoskun/cognitive_bias_ontology/main/misattributionOfMemory.owl#Social_Media">
        <rdf:type rdf:resource="https://raw.githubusercontent.com/ranacoskun/cognitive_bias_ontology/main/misattributionOfMemory.owl#OriginalSource"/>
        <rdfs:comment>Information found on a social media platform</rdfs:comment>
    </owl:NamedIndividual>
    


    <!-- https://raw.githubusercontent.com/ranacoskun/cognitive_bias_ontology/main/misattributionOfMemory.owl#book_plot -->

    <owl:NamedIndividual rdf:about="https://raw.githubusercontent.com/ranacoskun/cognitive_bias_ontology/main/misattributionOfMemory.owl#book_plot">
        <rdf:type rdf:resource="https://raw.githubusercontent.com/ranacoskun/cognitive_bias_ontology/main/cbi.owl#Cryptomnesia"/>
        <rdfs:comment>Original book plot that the writer forgot about</rdfs:comment>
        <rdfs:comment>The writer writes a book using a plot he found in a book he read years before without recalling</rdfs:comment>
    </owl:NamedIndividual>
    


    <!-- https://raw.githubusercontent.com/ranacoskun/cognitive_bias_ontology/main/misattributionOfMemory.owl#cross_examination_strategy -->

    <owl:NamedIndividual rdf:about="https://raw.githubusercontent.com/ranacoskun/cognitive_bias_ontology/main/misattributionOfMemory.owl#cross_examination_strategy">
        <rdf:type rdf:resource="https://raw.githubusercontent.com/ranacoskun/cognitive_bias_ontology/main/misattributionOfMemory.owl#MemoryTest"/>
        <rdfs:comment>Develop a series of questions for Jane Doe that highlight the conditions under which she observed the suspect (e.g., lighting, stress, distance, and her confidence in her recall). Emphasize factors that could have impaired her ability to accurately identify the defendant.</rdfs:comment>
    </owl:NamedIndividual>
    


    <!-- https://raw.githubusercontent.com/ranacoskun/cognitive_bias_ontology/main/misattributionOfMemory.owl#false_accusation -->

    <owl:NamedIndividual rdf:about="https://raw.githubusercontent.com/ranacoskun/cognitive_bias_ontology/main/misattributionOfMemory.owl#false_accusation">
        <rdf:type rdf:resource="https://raw.githubusercontent.com/ranacoskun/cognitive_bias_ontology/main/cbi.owl#FalseMemory"/>
        <rdfs:comment>The biased agent remembers incorrectly the appearance of a person seen during a robbery.</rdfs:comment>
    </owl:NamedIndividual>
    


    <!-- https://raw.githubusercontent.com/ranacoskun/cognitive_bias_ontology/main/misattributionOfMemory.owl#memory_point -->

    <owl:NamedIndividual rdf:about="https://raw.githubusercontent.com/ranacoskun/cognitive_bias_ontology/main/misattributionOfMemory.owl#memory_point">
        <rdf:type rdf:resource="https://raw.githubusercontent.com/ranacoskun/cognitive_bias_ontology/main/misattributionOfMemory.owl#CognitiveError"/>
        <rdfs:comment>construction of a false memory point, it&apos;s a common cognitive error</rdfs:comment>
    </owl:NamedIndividual>
    


    <!-- https://raw.githubusercontent.com/ranacoskun/cognitive_bias_ontology/main/misattributionOfMemory.owl#new_book_plot -->

    <owl:NamedIndividual rdf:about="https://raw.githubusercontent.com/ranacoskun/cognitive_bias_ontology/main/misattributionOfMemory.owl#new_book_plot">
        <rdf:type rdf:resource="https://raw.githubusercontent.com/ranacoskun/cognitive_bias_ontology/main/misattributionOfMemory.owl#RecalledIdea"/>
        <rdfs:comment>A plot for a new book from the writer</rdfs:comment>
    </owl:NamedIndividual>
    


    <!-- https://raw.githubusercontent.com/ranacoskun/cognitive_bias_ontology/main/misattributionOfMemory.owl#old_unknown_book -->

    <owl:NamedIndividual rdf:about="https://raw.githubusercontent.com/ranacoskun/cognitive_bias_ontology/main/misattributionOfMemory.owl#old_unknown_book">
        <rdf:type rdf:resource="https://raw.githubusercontent.com/ranacoskun/cognitive_bias_ontology/main/misattributionOfMemory.owl#OriginalSource"/>
        <rdfs:comment>Book that is presumably unknown from which the author inadvertedly copied the plot</rdfs:comment>
    </owl:NamedIndividual>
    


    <!-- https://raw.githubusercontent.com/ranacoskun/cognitive_bias_ontology/main/misattributionOfMemory.owl#reenactment -->

    <owl:NamedIndividual rdf:about="https://raw.githubusercontent.com/ranacoskun/cognitive_bias_ontology/main/misattributionOfMemory.owl#reenactment">
        <rdf:type rdf:resource="https://raw.githubusercontent.com/ranacoskun/cognitive_bias_ontology/main/misattributionOfMemory.owl#Correction"/>
        <rdfs:comment>Use visual aids or a reenactment to demonstrate to the jury the conditions under which the eyewitness made her observations, including any obstacles, lighting conditions, and the distance from which she viewed the suspect.</rdfs:comment>
    </owl:NamedIndividual>
    


    <!-- https://raw.githubusercontent.com/ranacoskun/cognitive_bias_ontology/main/misattributionOfMemory.owl#source_confusion_agent -->

    <owl:NamedIndividual rdf:about="https://raw.githubusercontent.com/ranacoskun/cognitive_bias_ontology/main/misattributionOfMemory.owl#source_confusion_agent">
        <rdf:type rdf:resource="https://raw.githubusercontent.com/ranacoskun/cognitive_bias_ontology/main/cbi.owl#BiasedAgent"/>
        <rdfs:comment>Person affected by the Source Confusion Bias</rdfs:comment>
    </owl:NamedIndividual>
    


    <!-- https://raw.githubusercontent.com/ranacoskun/cognitive_bias_ontology/main/misattributionOfMemory.owl#suggestive_questioning -->

    <owl:NamedIndividual rdf:about="https://raw.githubusercontent.com/ranacoskun/cognitive_bias_ontology/main/misattributionOfMemory.owl#suggestive_questioning">
        <rdf:type rdf:resource="https://raw.githubusercontent.com/ranacoskun/cognitive_bias_ontology/main/misattributionOfMemory.owl#Cause"/>
        <rdfs:comment>A suggestive question is one that implies that a certain answer should be given in response, or falsely presents a presupposition in the question as accepted fact.</rdfs:comment>
    </owl:NamedIndividual>
    


    <!-- https://raw.githubusercontent.com/ranacoskun/cognitive_bias_ontology/main/misattributionOfMemory.owl#writer -->

    <owl:NamedIndividual rdf:about="https://raw.githubusercontent.com/ranacoskun/cognitive_bias_ontology/main/misattributionOfMemory.owl#writer">
        <rdf:type rdf:resource="https://raw.githubusercontent.com/ranacoskun/cognitive_bias_ontology/main/cbi.owl#BiasedAgent"/>
        <rdfs:comment>Writer who doesn&apos;t recall a book that read many years ago</rdfs:comment>
    </owl:NamedIndividual>
    


    <!-- https://raw.githubusercontent.com/ranacoskun/cognitive_bias_ontology/main/misattributionOfMemory.owl#wrongful_detention -->

    <owl:NamedIndividual rdf:about="https://raw.githubusercontent.com/ranacoskun/cognitive_bias_ontology/main/misattributionOfMemory.owl#wrongful_detention">
        <rdf:type rdf:resource="https://raw.githubusercontent.com/ranacoskun/cognitive_bias_ontology/main/misattributionOfMemory.owl#Effect"/>
        <rdfs:comment>The biased testimony results in the arrest of John Smith</rdfs:comment>
    </owl:NamedIndividual>
    


    <!-- 
    ///////////////////////////////////////////////////////////////////////////////////////
    //
    // General axioms
    //
    ///////////////////////////////////////////////////////////////////////////////////////
     -->

    <rdf:Description>
        <rdf:type rdf:resource="http://www.w3.org/2002/07/owl#AllDisjointClasses"/>
        <owl:members rdf:parseType="Collection">
            <rdf:Description rdf:about="https://raw.githubusercontent.com/ranacoskun/cognitive_bias_ontology/main/cbi.owl#Cryptomnesia"/>
            <rdf:Description rdf:about="https://raw.githubusercontent.com/ranacoskun/cognitive_bias_ontology/main/cbi.owl#FalseMemory"/>
            <rdf:Description rdf:about="https://raw.githubusercontent.com/ranacoskun/cognitive_bias_ontology/main/cbi.owl#SourceConfusion"/>
        </owl:members>
    </rdf:Description>
</rdf:RDF>



<!-- Generated by the OWL API (version 4.5.29.2024-05-13T12:11:03Z) https://github.com/owlcs/owlapi -->

