Prefix(:=<https://raw.githubusercontent.com/ranacoskun/cognitive_bias_ontology/main/misattributionOfMemory.owl>)
Prefix(cbi:=<https://raw.githubusercontent.com/ranacoskun/cognitive_bias_ontology/main/cbi.owl>)
Prefix(mom:=<https://raw.githubusercontent.com/ranacoskun/cognitive_bias_ontology/main/misattributionOfMemory.owl>)
Prefix(owl:=<http://www.w3.org/2002/07/owl#>)
Prefix(rdf:=<http://www.w3.org/1999/02/22-rdf-syntax-ns#>)
Prefix(xml:=<http://www.w3.org/XML/1998/namespace>)
Prefix(xsd:=<http://www.w3.org/2001/XMLSchema#>)
Prefix(rdfs:=<http://www.w3.org/2000/01/rdf-schema#>)


Ontology(<https://raw.githubusercontent.com/ranacoskun/cognitive_bias_ontology/main/misattributionOfMemory.owl>
Annotation(<http://purl.org/dc/elements/1.1/creator> "Francesco Alaimo")
Annotation(<http://purl.org/dc/elements/1.1/title> "Misattribution of memory")
Annotation(rdfs:comment "This is an ontology that describes the behaviour of a person affected by the Misattribution of memory bias.")

Declaration(Class(<http://etna.istc.cnr.it/framester2/data/framestercore/Event>))
Declaration(Class(<http://etna.istc.cnr.it/framester2/data/framestercore/Memorization>))
Declaration(Class(<http://etna.istc.cnr.it/framester2/data/framestercore/People>))
Declaration(Class(<https://dbpedia.org/ontology/Media>))
Declaration(Class(<https://raw.githubusercontent.com/ranacoskun/cognitive_bias_ontology/main/cbi.owl#BiasedAgent>))
Declaration(Class(<https://raw.githubusercontent.com/ranacoskun/cognitive_bias_ontology/main/cbi.owl#CognitiveBias>))
Declaration(Class(<https://raw.githubusercontent.com/ranacoskun/cognitive_bias_ontology/main/misattributionOfMemory.owl#Cause>))
Declaration(Class(<https://raw.githubusercontent.com/ranacoskun/cognitive_bias_ontology/main/misattributionOfMemory.owl#CognitiveError>))
Declaration(Class(<https://raw.githubusercontent.com/ranacoskun/cognitive_bias_ontology/main/misattributionOfMemory.owl#Correction>))
Declaration(Class(<https://raw.githubusercontent.com/ranacoskun/cognitive_bias_ontology/main/misattributionOfMemory.owl#Cryptomnesia>))
Declaration(Class(<https://raw.githubusercontent.com/ranacoskun/cognitive_bias_ontology/main/misattributionOfMemory.owl#Effect>))
Declaration(Class(<https://raw.githubusercontent.com/ranacoskun/cognitive_bias_ontology/main/misattributionOfMemory.owl#Evidence>))
Declaration(Class(<https://raw.githubusercontent.com/ranacoskun/cognitive_bias_ontology/main/misattributionOfMemory.owl#FalseMemory>))
Declaration(Class(<https://raw.githubusercontent.com/ranacoskun/cognitive_bias_ontology/main/misattributionOfMemory.owl#MemoryTest>))
Declaration(Class(<https://raw.githubusercontent.com/ranacoskun/cognitive_bias_ontology/main/misattributionOfMemory.owl#MisattributedMemory>))
Declaration(Class(<https://raw.githubusercontent.com/ranacoskun/cognitive_bias_ontology/main/misattributionOfMemory.owl#OriginalSource>))
Declaration(Class(<https://raw.githubusercontent.com/ranacoskun/cognitive_bias_ontology/main/misattributionOfMemory.owl#Prevention>))
Declaration(Class(<https://raw.githubusercontent.com/ranacoskun/cognitive_bias_ontology/main/misattributionOfMemory.owl#RecalledIdea>))
Declaration(Class(<https://raw.githubusercontent.com/ranacoskun/cognitive_bias_ontology/main/misattributionOfMemory.owl#SourceConfusion>))
Declaration(ObjectProperty(<https://raw.githubusercontent.com/ranacoskun/cognitive_bias_ontology/main/misattributionOfMemory.owl#affects>))
Declaration(ObjectProperty(<https://raw.githubusercontent.com/ranacoskun/cognitive_bias_ontology/main/misattributionOfMemory.owl#canBeCorrectedBy>))
Declaration(ObjectProperty(<https://raw.githubusercontent.com/ranacoskun/cognitive_bias_ontology/main/misattributionOfMemory.owl#canBePreventedBy>))
Declaration(ObjectProperty(<https://raw.githubusercontent.com/ranacoskun/cognitive_bias_ontology/main/misattributionOfMemory.owl#creates>))
Declaration(ObjectProperty(<https://raw.githubusercontent.com/ranacoskun/cognitive_bias_ontology/main/misattributionOfMemory.owl#forgets>))
Declaration(ObjectProperty(<https://raw.githubusercontent.com/ranacoskun/cognitive_bias_ontology/main/misattributionOfMemory.owl#generatedBy>))
Declaration(ObjectProperty(<https://raw.githubusercontent.com/ranacoskun/cognitive_bias_ontology/main/misattributionOfMemory.owl#hasCause>))
Declaration(ObjectProperty(<https://raw.githubusercontent.com/ranacoskun/cognitive_bias_ontology/main/misattributionOfMemory.owl#hasEffect>))
Declaration(ObjectProperty(<https://raw.githubusercontent.com/ranacoskun/cognitive_bias_ontology/main/misattributionOfMemory.owl#hasParticipant>))
Declaration(ObjectProperty(<https://raw.githubusercontent.com/ranacoskun/cognitive_bias_ontology/main/misattributionOfMemory.owl#isAffectedBy>))
Declaration(ObjectProperty(<https://raw.githubusercontent.com/ranacoskun/cognitive_bias_ontology/main/misattributionOfMemory.owl#isAssessedBy>))
Declaration(ObjectProperty(<https://raw.githubusercontent.com/ranacoskun/cognitive_bias_ontology/main/misattributionOfMemory.owl#isDerivedFrom>))
Declaration(ObjectProperty(<https://raw.githubusercontent.com/ranacoskun/cognitive_bias_ontology/main/misattributionOfMemory.owl#isRecalledIn>))
Declaration(ObjectProperty(<https://raw.githubusercontent.com/ranacoskun/cognitive_bias_ontology/main/misattributionOfMemory.owl#isSupportedOrRefutedBy>))
Declaration(ObjectProperty(<https://raw.githubusercontent.com/ranacoskun/cognitive_bias_ontology/main/misattributionOfMemory.owl#leadsTo>))
Declaration(ObjectProperty(<https://raw.githubusercontent.com/ranacoskun/cognitive_bias_ontology/main/misattributionOfMemory.owl#occursIn>))
Declaration(ObjectProperty(<https://raw.githubusercontent.com/ranacoskun/cognitive_bias_ontology/main/misattributionOfMemory.owl#relatesToEvent>))
Declaration(NamedIndividual(<https://raw.githubusercontent.com/ranacoskun/cognitive_bias_ontology/main/misattributionOfMemory.owl#CCTV_footage>))
Declaration(NamedIndividual(<https://raw.githubusercontent.com/ranacoskun/cognitive_bias_ontology/main/misattributionOfMemory.owl#Jane_Doe>))
Declaration(NamedIndividual(<https://raw.githubusercontent.com/ranacoskun/cognitive_bias_ontology/main/misattributionOfMemory.owl#cross_examination_strategy>))
Declaration(NamedIndividual(<https://raw.githubusercontent.com/ranacoskun/cognitive_bias_ontology/main/misattributionOfMemory.owl#false_accusation>))
Declaration(NamedIndividual(<https://raw.githubusercontent.com/ranacoskun/cognitive_bias_ontology/main/misattributionOfMemory.owl#reenactment>))
Declaration(NamedIndividual(<https://raw.githubusercontent.com/ranacoskun/cognitive_bias_ontology/main/misattributionOfMemory.owl#suggestive_questioning>))
Declaration(NamedIndividual(<https://raw.githubusercontent.com/ranacoskun/cognitive_bias_ontology/main/misattributionOfMemory.owl#wrongful_detention>))
Declaration(AnnotationProperty(<http://purl.org/dc/elements/1.1/creator>))
Declaration(AnnotationProperty(<http://purl.org/dc/elements/1.1/title>))
Declaration(AnnotationProperty(rdfs:label))

############################
#   Object Properties
############################

# Object Property: <https://raw.githubusercontent.com/ranacoskun/cognitive_bias_ontology/main/misattributionOfMemory.owl#affects> (<https://raw.githubusercontent.com/ranacoskun/cognitive_bias_ontology/main/misattributionOfMemory.owl#affects>)

SubObjectPropertyOf(<https://raw.githubusercontent.com/ranacoskun/cognitive_bias_ontology/main/misattributionOfMemory.owl#affects> owl:topObjectProperty)
InverseObjectProperties(<https://raw.githubusercontent.com/ranacoskun/cognitive_bias_ontology/main/misattributionOfMemory.owl#affects> <https://raw.githubusercontent.com/ranacoskun/cognitive_bias_ontology/main/misattributionOfMemory.owl#isAffectedBy>)
ObjectPropertyDomain(<https://raw.githubusercontent.com/ranacoskun/cognitive_bias_ontology/main/misattributionOfMemory.owl#affects> <https://raw.githubusercontent.com/ranacoskun/cognitive_bias_ontology/main/misattributionOfMemory.owl#Cryptomnesia>)
ObjectPropertyDomain(<https://raw.githubusercontent.com/ranacoskun/cognitive_bias_ontology/main/misattributionOfMemory.owl#affects> <https://raw.githubusercontent.com/ranacoskun/cognitive_bias_ontology/main/misattributionOfMemory.owl#FalseMemory>)
ObjectPropertyDomain(<https://raw.githubusercontent.com/ranacoskun/cognitive_bias_ontology/main/misattributionOfMemory.owl#affects> <https://raw.githubusercontent.com/ranacoskun/cognitive_bias_ontology/main/misattributionOfMemory.owl#SourceConfusion>)
ObjectPropertyRange(<https://raw.githubusercontent.com/ranacoskun/cognitive_bias_ontology/main/misattributionOfMemory.owl#affects> <https://raw.githubusercontent.com/ranacoskun/cognitive_bias_ontology/main/cbi.owl#BiasedAgent>)

# Object Property: <https://raw.githubusercontent.com/ranacoskun/cognitive_bias_ontology/main/misattributionOfMemory.owl#canBeCorrectedBy> (<https://raw.githubusercontent.com/ranacoskun/cognitive_bias_ontology/main/misattributionOfMemory.owl#canBeCorrectedBy>)

AnnotationAssertion(rdfs:comment <https://raw.githubusercontent.com/ranacoskun/cognitive_bias_ontology/main/misattributionOfMemory.owl#canBeCorrectedBy> "Describes the relation between the bias and the correction to enact")
ObjectPropertyDomain(<https://raw.githubusercontent.com/ranacoskun/cognitive_bias_ontology/main/misattributionOfMemory.owl#canBeCorrectedBy> <https://raw.githubusercontent.com/ranacoskun/cognitive_bias_ontology/main/misattributionOfMemory.owl#FalseMemory>)
ObjectPropertyRange(<https://raw.githubusercontent.com/ranacoskun/cognitive_bias_ontology/main/misattributionOfMemory.owl#canBeCorrectedBy> <https://raw.githubusercontent.com/ranacoskun/cognitive_bias_ontology/main/misattributionOfMemory.owl#Correction>)

# Object Property: <https://raw.githubusercontent.com/ranacoskun/cognitive_bias_ontology/main/misattributionOfMemory.owl#canBePreventedBy> (<https://raw.githubusercontent.com/ranacoskun/cognitive_bias_ontology/main/misattributionOfMemory.owl#canBePreventedBy>)

AnnotationAssertion(rdfs:comment <https://raw.githubusercontent.com/ranacoskun/cognitive_bias_ontology/main/misattributionOfMemory.owl#canBePreventedBy> "Describes the relation between the bias and the prevention techniques to it")
ObjectPropertyDomain(<https://raw.githubusercontent.com/ranacoskun/cognitive_bias_ontology/main/misattributionOfMemory.owl#canBePreventedBy> <https://raw.githubusercontent.com/ranacoskun/cognitive_bias_ontology/main/misattributionOfMemory.owl#FalseMemory>)
ObjectPropertyRange(<https://raw.githubusercontent.com/ranacoskun/cognitive_bias_ontology/main/misattributionOfMemory.owl#canBePreventedBy> <https://raw.githubusercontent.com/ranacoskun/cognitive_bias_ontology/main/misattributionOfMemory.owl#Prevention>)

# Object Property: <https://raw.githubusercontent.com/ranacoskun/cognitive_bias_ontology/main/misattributionOfMemory.owl#creates> (<https://raw.githubusercontent.com/ranacoskun/cognitive_bias_ontology/main/misattributionOfMemory.owl#creates>)

AnnotationAssertion(rdfs:comment <https://raw.githubusercontent.com/ranacoskun/cognitive_bias_ontology/main/misattributionOfMemory.owl#creates> "Creates the relation between the person affected by the bias and the creation of a self assessed original creation")
ObjectPropertyDomain(<https://raw.githubusercontent.com/ranacoskun/cognitive_bias_ontology/main/misattributionOfMemory.owl#creates> <http://etna.istc.cnr.it/framester2/data/framestercore/People>)
ObjectPropertyRange(<https://raw.githubusercontent.com/ranacoskun/cognitive_bias_ontology/main/misattributionOfMemory.owl#creates> <https://raw.githubusercontent.com/ranacoskun/cognitive_bias_ontology/main/misattributionOfMemory.owl#RecalledIdea>)

# Object Property: <https://raw.githubusercontent.com/ranacoskun/cognitive_bias_ontology/main/misattributionOfMemory.owl#forgets> (<https://raw.githubusercontent.com/ranacoskun/cognitive_bias_ontology/main/misattributionOfMemory.owl#forgets>)

AnnotationAssertion(rdfs:comment <https://raw.githubusercontent.com/ranacoskun/cognitive_bias_ontology/main/misattributionOfMemory.owl#forgets> "Describes the lost of memory from the biased agents towards the Original Source")
ObjectPropertyDomain(<https://raw.githubusercontent.com/ranacoskun/cognitive_bias_ontology/main/misattributionOfMemory.owl#forgets> <http://etna.istc.cnr.it/framester2/data/framestercore/People>)
ObjectPropertyRange(<https://raw.githubusercontent.com/ranacoskun/cognitive_bias_ontology/main/misattributionOfMemory.owl#forgets> <https://raw.githubusercontent.com/ranacoskun/cognitive_bias_ontology/main/misattributionOfMemory.owl#OriginalSource>)

# Object Property: <https://raw.githubusercontent.com/ranacoskun/cognitive_bias_ontology/main/misattributionOfMemory.owl#generatedBy> (<https://raw.githubusercontent.com/ranacoskun/cognitive_bias_ontology/main/misattributionOfMemory.owl#generatedBy>)

AnnotationAssertion(rdfs:comment <https://raw.githubusercontent.com/ranacoskun/cognitive_bias_ontology/main/misattributionOfMemory.owl#generatedBy> "Describes the relation between a bias and the source from which it starts or come from")
ObjectPropertyDomain(<https://raw.githubusercontent.com/ranacoskun/cognitive_bias_ontology/main/misattributionOfMemory.owl#generatedBy> ObjectUnionOf(<http://etna.istc.cnr.it/framester2/data/framestercore/Memorization> <https://raw.githubusercontent.com/ranacoskun/cognitive_bias_ontology/main/misattributionOfMemory.owl#SourceConfusion>))
ObjectPropertyRange(<https://raw.githubusercontent.com/ranacoskun/cognitive_bias_ontology/main/misattributionOfMemory.owl#generatedBy> <http://etna.istc.cnr.it/framester2/data/framestercore/Event>)
ObjectPropertyRange(<https://raw.githubusercontent.com/ranacoskun/cognitive_bias_ontology/main/misattributionOfMemory.owl#generatedBy> <https://raw.githubusercontent.com/ranacoskun/cognitive_bias_ontology/main/misattributionOfMemory.owl#OriginalSource>)

# Object Property: <https://raw.githubusercontent.com/ranacoskun/cognitive_bias_ontology/main/misattributionOfMemory.owl#hasCause> (<https://raw.githubusercontent.com/ranacoskun/cognitive_bias_ontology/main/misattributionOfMemory.owl#hasCause>)

AnnotationAssertion(rdfs:comment <https://raw.githubusercontent.com/ranacoskun/cognitive_bias_ontology/main/misattributionOfMemory.owl#hasCause> "Describes the relation between the a Bias and its inherent cause")
ObjectPropertyDomain(<https://raw.githubusercontent.com/ranacoskun/cognitive_bias_ontology/main/misattributionOfMemory.owl#hasCause> <https://raw.githubusercontent.com/ranacoskun/cognitive_bias_ontology/main/misattributionOfMemory.owl#FalseMemory>)
ObjectPropertyRange(<https://raw.githubusercontent.com/ranacoskun/cognitive_bias_ontology/main/misattributionOfMemory.owl#hasCause> <https://raw.githubusercontent.com/ranacoskun/cognitive_bias_ontology/main/misattributionOfMemory.owl#Cause>)

# Object Property: <https://raw.githubusercontent.com/ranacoskun/cognitive_bias_ontology/main/misattributionOfMemory.owl#hasEffect> (<https://raw.githubusercontent.com/ranacoskun/cognitive_bias_ontology/main/misattributionOfMemory.owl#hasEffect>)

AnnotationAssertion(rdfs:comment <https://raw.githubusercontent.com/ranacoskun/cognitive_bias_ontology/main/misattributionOfMemory.owl#hasEffect> "Describes the relation between the bias and its effect")
ObjectPropertyDomain(<https://raw.githubusercontent.com/ranacoskun/cognitive_bias_ontology/main/misattributionOfMemory.owl#hasEffect> <https://raw.githubusercontent.com/ranacoskun/cognitive_bias_ontology/main/misattributionOfMemory.owl#FalseMemory>)
ObjectPropertyRange(<https://raw.githubusercontent.com/ranacoskun/cognitive_bias_ontology/main/misattributionOfMemory.owl#hasEffect> <https://raw.githubusercontent.com/ranacoskun/cognitive_bias_ontology/main/misattributionOfMemory.owl#Effect>)

# Object Property: <https://raw.githubusercontent.com/ranacoskun/cognitive_bias_ontology/main/misattributionOfMemory.owl#hasParticipant> (<https://raw.githubusercontent.com/ranacoskun/cognitive_bias_ontology/main/misattributionOfMemory.owl#hasParticipant>)

AnnotationAssertion(rdfs:comment <https://raw.githubusercontent.com/ranacoskun/cognitive_bias_ontology/main/misattributionOfMemory.owl#hasParticipant> "Describes the relation between the Event and the Biased Agent who participate")
ObjectPropertyDomain(<https://raw.githubusercontent.com/ranacoskun/cognitive_bias_ontology/main/misattributionOfMemory.owl#hasParticipant> <http://etna.istc.cnr.it/framester2/data/framestercore/Event>)
ObjectPropertyDomain(<https://raw.githubusercontent.com/ranacoskun/cognitive_bias_ontology/main/misattributionOfMemory.owl#hasParticipant> <https://raw.githubusercontent.com/ranacoskun/cognitive_bias_ontology/main/misattributionOfMemory.owl#CognitiveError>)
ObjectPropertyRange(<https://raw.githubusercontent.com/ranacoskun/cognitive_bias_ontology/main/misattributionOfMemory.owl#hasParticipant> <http://etna.istc.cnr.it/framester2/data/framestercore/People>)

# Object Property: <https://raw.githubusercontent.com/ranacoskun/cognitive_bias_ontology/main/misattributionOfMemory.owl#isAffectedBy> (<https://raw.githubusercontent.com/ranacoskun/cognitive_bias_ontology/main/misattributionOfMemory.owl#isAffectedBy>)

AnnotationAssertion(rdfs:comment <https://raw.githubusercontent.com/ranacoskun/cognitive_bias_ontology/main/misattributionOfMemory.owl#isAffectedBy> "Describes the relationship between Biased Agent and Bias")
ObjectPropertyDomain(<https://raw.githubusercontent.com/ranacoskun/cognitive_bias_ontology/main/misattributionOfMemory.owl#isAffectedBy> <https://raw.githubusercontent.com/ranacoskun/cognitive_bias_ontology/main/cbi.owl#BiasedAgent>)
ObjectPropertyRange(<https://raw.githubusercontent.com/ranacoskun/cognitive_bias_ontology/main/misattributionOfMemory.owl#isAffectedBy> <https://raw.githubusercontent.com/ranacoskun/cognitive_bias_ontology/main/misattributionOfMemory.owl#Cryptomnesia>)
ObjectPropertyRange(<https://raw.githubusercontent.com/ranacoskun/cognitive_bias_ontology/main/misattributionOfMemory.owl#isAffectedBy> <https://raw.githubusercontent.com/ranacoskun/cognitive_bias_ontology/main/misattributionOfMemory.owl#FalseMemory>)
ObjectPropertyRange(<https://raw.githubusercontent.com/ranacoskun/cognitive_bias_ontology/main/misattributionOfMemory.owl#isAffectedBy> <https://raw.githubusercontent.com/ranacoskun/cognitive_bias_ontology/main/misattributionOfMemory.owl#SourceConfusion>)

# Object Property: <https://raw.githubusercontent.com/ranacoskun/cognitive_bias_ontology/main/misattributionOfMemory.owl#isAssessedBy> (<https://raw.githubusercontent.com/ranacoskun/cognitive_bias_ontology/main/misattributionOfMemory.owl#isAssessedBy>)

AnnotationAssertion(rdfs:comment <https://raw.githubusercontent.com/ranacoskun/cognitive_bias_ontology/main/misattributionOfMemory.owl#isAssessedBy> "Describes the relation between the bias and the Memory Test")
ObjectPropertyDomain(<https://raw.githubusercontent.com/ranacoskun/cognitive_bias_ontology/main/misattributionOfMemory.owl#isAssessedBy> <https://raw.githubusercontent.com/ranacoskun/cognitive_bias_ontology/main/misattributionOfMemory.owl#FalseMemory>)
ObjectPropertyRange(<https://raw.githubusercontent.com/ranacoskun/cognitive_bias_ontology/main/misattributionOfMemory.owl#isAssessedBy> <https://raw.githubusercontent.com/ranacoskun/cognitive_bias_ontology/main/misattributionOfMemory.owl#MemoryTest>)

# Object Property: <https://raw.githubusercontent.com/ranacoskun/cognitive_bias_ontology/main/misattributionOfMemory.owl#isDerivedFrom> (<https://raw.githubusercontent.com/ranacoskun/cognitive_bias_ontology/main/misattributionOfMemory.owl#isDerivedFrom>)

AnnotationAssertion(rdfs:comment <https://raw.githubusercontent.com/ranacoskun/cognitive_bias_ontology/main/misattributionOfMemory.owl#isDerivedFrom> "Puts in relation the self assessed original creation and the true original source of it")
ObjectPropertyDomain(<https://raw.githubusercontent.com/ranacoskun/cognitive_bias_ontology/main/misattributionOfMemory.owl#isDerivedFrom> <https://raw.githubusercontent.com/ranacoskun/cognitive_bias_ontology/main/misattributionOfMemory.owl#RecalledIdea>)
ObjectPropertyRange(<https://raw.githubusercontent.com/ranacoskun/cognitive_bias_ontology/main/misattributionOfMemory.owl#isDerivedFrom> <https://raw.githubusercontent.com/ranacoskun/cognitive_bias_ontology/main/misattributionOfMemory.owl#OriginalSource>)

# Object Property: <https://raw.githubusercontent.com/ranacoskun/cognitive_bias_ontology/main/misattributionOfMemory.owl#isRecalledIn> (<https://raw.githubusercontent.com/ranacoskun/cognitive_bias_ontology/main/misattributionOfMemory.owl#isRecalledIn>)

AnnotationAssertion(rdfs:comment <https://raw.githubusercontent.com/ranacoskun/cognitive_bias_ontology/main/misattributionOfMemory.owl#isRecalledIn> "Describes the relation between the original source and the current Bias")
ObjectPropertyDomain(<https://raw.githubusercontent.com/ranacoskun/cognitive_bias_ontology/main/misattributionOfMemory.owl#isRecalledIn> <https://raw.githubusercontent.com/ranacoskun/cognitive_bias_ontology/main/misattributionOfMemory.owl#OriginalSource>)
ObjectPropertyRange(<https://raw.githubusercontent.com/ranacoskun/cognitive_bias_ontology/main/misattributionOfMemory.owl#isRecalledIn> <https://raw.githubusercontent.com/ranacoskun/cognitive_bias_ontology/main/misattributionOfMemory.owl#Cryptomnesia>)

# Object Property: <https://raw.githubusercontent.com/ranacoskun/cognitive_bias_ontology/main/misattributionOfMemory.owl#isSupportedOrRefutedBy> (<https://raw.githubusercontent.com/ranacoskun/cognitive_bias_ontology/main/misattributionOfMemory.owl#isSupportedOrRefutedBy>)

AnnotationAssertion(rdfs:comment <https://raw.githubusercontent.com/ranacoskun/cognitive_bias_ontology/main/misattributionOfMemory.owl#isSupportedOrRefutedBy> "Describes the relation between the False Memory and the Evidence")
ObjectPropertyDomain(<https://raw.githubusercontent.com/ranacoskun/cognitive_bias_ontology/main/misattributionOfMemory.owl#isSupportedOrRefutedBy> <https://raw.githubusercontent.com/ranacoskun/cognitive_bias_ontology/main/misattributionOfMemory.owl#FalseMemory>)
ObjectPropertyRange(<https://raw.githubusercontent.com/ranacoskun/cognitive_bias_ontology/main/misattributionOfMemory.owl#isSupportedOrRefutedBy> <https://raw.githubusercontent.com/ranacoskun/cognitive_bias_ontology/main/misattributionOfMemory.owl#Evidence>)

# Object Property: <https://raw.githubusercontent.com/ranacoskun/cognitive_bias_ontology/main/misattributionOfMemory.owl#leadsTo> (<https://raw.githubusercontent.com/ranacoskun/cognitive_bias_ontology/main/misattributionOfMemory.owl#leadsTo>)

AnnotationAssertion(rdfs:comment <https://raw.githubusercontent.com/ranacoskun/cognitive_bias_ontology/main/misattributionOfMemory.owl#leadsTo> "Describes the relation between the cognitive error and the bias")
ObjectPropertyDomain(<https://raw.githubusercontent.com/ranacoskun/cognitive_bias_ontology/main/misattributionOfMemory.owl#leadsTo> <https://raw.githubusercontent.com/ranacoskun/cognitive_bias_ontology/main/misattributionOfMemory.owl#CognitiveError>)
ObjectPropertyRange(<https://raw.githubusercontent.com/ranacoskun/cognitive_bias_ontology/main/misattributionOfMemory.owl#leadsTo> <https://raw.githubusercontent.com/ranacoskun/cognitive_bias_ontology/main/misattributionOfMemory.owl#SourceConfusion>)

# Object Property: <https://raw.githubusercontent.com/ranacoskun/cognitive_bias_ontology/main/misattributionOfMemory.owl#occursIn> (<https://raw.githubusercontent.com/ranacoskun/cognitive_bias_ontology/main/misattributionOfMemory.owl#occursIn>)

AnnotationAssertion(rdfs:comment <https://raw.githubusercontent.com/ranacoskun/cognitive_bias_ontology/main/misattributionOfMemory.owl#occursIn> "Puts in relation the current Bias and the Media through which it can be exposed")
ObjectPropertyDomain(<https://raw.githubusercontent.com/ranacoskun/cognitive_bias_ontology/main/misattributionOfMemory.owl#occursIn> <https://raw.githubusercontent.com/ranacoskun/cognitive_bias_ontology/main/misattributionOfMemory.owl#Cryptomnesia>)
ObjectPropertyRange(<https://raw.githubusercontent.com/ranacoskun/cognitive_bias_ontology/main/misattributionOfMemory.owl#occursIn> <https://dbpedia.org/ontology/Media>)

# Object Property: <https://raw.githubusercontent.com/ranacoskun/cognitive_bias_ontology/main/misattributionOfMemory.owl#relatesToEvent> (<https://raw.githubusercontent.com/ranacoskun/cognitive_bias_ontology/main/misattributionOfMemory.owl#relatesToEvent>)

AnnotationAssertion(rdfs:comment <https://raw.githubusercontent.com/ranacoskun/cognitive_bias_ontology/main/misattributionOfMemory.owl#relatesToEvent> "Describes the relation between the Cognitive Error committed and the Event in which it takes place")
ObjectPropertyDomain(<https://raw.githubusercontent.com/ranacoskun/cognitive_bias_ontology/main/misattributionOfMemory.owl#relatesToEvent> <https://raw.githubusercontent.com/ranacoskun/cognitive_bias_ontology/main/misattributionOfMemory.owl#CognitiveError>)
ObjectPropertyRange(<https://raw.githubusercontent.com/ranacoskun/cognitive_bias_ontology/main/misattributionOfMemory.owl#relatesToEvent> <http://etna.istc.cnr.it/framester2/data/framestercore/Event>)



############################
#   Classes
############################

# Class: <https://raw.githubusercontent.com/ranacoskun/cognitive_bias_ontology/main/cbi.owl#BiasedAgent> (<https://raw.githubusercontent.com/ranacoskun/cognitive_bias_ontology/main/cbi.owl#BiasedAgent>)

AnnotationAssertion(rdfs:comment <https://raw.githubusercontent.com/ranacoskun/cognitive_bias_ontology/main/cbi.owl#BiasedAgent> "Represents an entity that experiences the bias.")
SubClassOf(<https://raw.githubusercontent.com/ranacoskun/cognitive_bias_ontology/main/cbi.owl#BiasedAgent> <http://etna.istc.cnr.it/framester2/data/framestercore/People>)

# Class: <https://raw.githubusercontent.com/ranacoskun/cognitive_bias_ontology/main/cbi.owl#CognitiveBias> (<https://raw.githubusercontent.com/ranacoskun/cognitive_bias_ontology/main/cbi.owl#CognitiveBias>)

AnnotationAssertion(rdfs:comment <https://raw.githubusercontent.com/ranacoskun/cognitive_bias_ontology/main/cbi.owl#CognitiveBias> "Represents the overarching concept of cognitive biases.")

# Class: <https://raw.githubusercontent.com/ranacoskun/cognitive_bias_ontology/main/misattributionOfMemory.owl#Cause> (<https://raw.githubusercontent.com/ranacoskun/cognitive_bias_ontology/main/misattributionOfMemory.owl#Cause>)

AnnotationAssertion(rdfs:comment <https://raw.githubusercontent.com/ranacoskun/cognitive_bias_ontology/main/misattributionOfMemory.owl#Cause> "Factors that contribute to the formation of false memories")

# Class: <https://raw.githubusercontent.com/ranacoskun/cognitive_bias_ontology/main/misattributionOfMemory.owl#CognitiveError> (<https://raw.githubusercontent.com/ranacoskun/cognitive_bias_ontology/main/misattributionOfMemory.owl#CognitiveError>)

AnnotationAssertion(rdfs:comment <https://raw.githubusercontent.com/ranacoskun/cognitive_bias_ontology/main/misattributionOfMemory.owl#CognitiveError> "A Cognitive error that leads to the Source Confusion bias, occurred during memorization")

# Class: <https://raw.githubusercontent.com/ranacoskun/cognitive_bias_ontology/main/misattributionOfMemory.owl#Correction> (<https://raw.githubusercontent.com/ranacoskun/cognitive_bias_ontology/main/misattributionOfMemory.owl#Correction>)

AnnotationAssertion(rdfs:comment <https://raw.githubusercontent.com/ranacoskun/cognitive_bias_ontology/main/misattributionOfMemory.owl#Correction> "Methods used to identify and correct false memories.")

# Class: <https://raw.githubusercontent.com/ranacoskun/cognitive_bias_ontology/main/misattributionOfMemory.owl#Cryptomnesia> (<https://raw.githubusercontent.com/ranacoskun/cognitive_bias_ontology/main/misattributionOfMemory.owl#Cryptomnesia>)

AnnotationAssertion(rdfs:comment <https://raw.githubusercontent.com/ranacoskun/cognitive_bias_ontology/main/misattributionOfMemory.owl#Cryptomnesia> "Describes the occurence of the Cryptomnesia bias")
SubClassOf(<https://raw.githubusercontent.com/ranacoskun/cognitive_bias_ontology/main/misattributionOfMemory.owl#Cryptomnesia> <https://raw.githubusercontent.com/ranacoskun/cognitive_bias_ontology/main/misattributionOfMemory.owl#MisattributedMemory>)

# Class: <https://raw.githubusercontent.com/ranacoskun/cognitive_bias_ontology/main/misattributionOfMemory.owl#Effect> (<https://raw.githubusercontent.com/ranacoskun/cognitive_bias_ontology/main/misattributionOfMemory.owl#Effect>)

AnnotationAssertion(rdfs:comment <https://raw.githubusercontent.com/ranacoskun/cognitive_bias_ontology/main/misattributionOfMemory.owl#Effect> "The impact or consequences of false memories on individuals and society.")

# Class: <https://raw.githubusercontent.com/ranacoskun/cognitive_bias_ontology/main/misattributionOfMemory.owl#Evidence> (<https://raw.githubusercontent.com/ranacoskun/cognitive_bias_ontology/main/misattributionOfMemory.owl#Evidence>)

AnnotationAssertion(rdfs:comment <https://raw.githubusercontent.com/ranacoskun/cognitive_bias_ontology/main/misattributionOfMemory.owl#Evidence> "Information or data used to support or refute the accuracy of a memory.")

# Class: <https://raw.githubusercontent.com/ranacoskun/cognitive_bias_ontology/main/misattributionOfMemory.owl#FalseMemory> (<https://raw.githubusercontent.com/ranacoskun/cognitive_bias_ontology/main/misattributionOfMemory.owl#FalseMemory>)

AnnotationAssertion(rdfs:comment <https://raw.githubusercontent.com/ranacoskun/cognitive_bias_ontology/main/misattributionOfMemory.owl#FalseMemory> "Describes the False Memory bias occurrence")
SubClassOf(<https://raw.githubusercontent.com/ranacoskun/cognitive_bias_ontology/main/misattributionOfMemory.owl#FalseMemory> <https://raw.githubusercontent.com/ranacoskun/cognitive_bias_ontology/main/misattributionOfMemory.owl#MisattributedMemory>)

# Class: <https://raw.githubusercontent.com/ranacoskun/cognitive_bias_ontology/main/misattributionOfMemory.owl#MemoryTest> (<https://raw.githubusercontent.com/ranacoskun/cognitive_bias_ontology/main/misattributionOfMemory.owl#MemoryTest>)

AnnotationAssertion(rdfs:comment <https://raw.githubusercontent.com/ranacoskun/cognitive_bias_ontology/main/misattributionOfMemory.owl#MemoryTest> "Tools or techniques used to assess the accuracy of memories and identify false ones")

# Class: <https://raw.githubusercontent.com/ranacoskun/cognitive_bias_ontology/main/misattributionOfMemory.owl#MisattributedMemory> (<https://raw.githubusercontent.com/ranacoskun/cognitive_bias_ontology/main/misattributionOfMemory.owl#MisattributedMemory>)

AnnotationAssertion(rdfs:comment <https://raw.githubusercontent.com/ranacoskun/cognitive_bias_ontology/main/misattributionOfMemory.owl#MisattributedMemory> "Describes a generic Misattribution of Memory")
SubClassOf(<https://raw.githubusercontent.com/ranacoskun/cognitive_bias_ontology/main/misattributionOfMemory.owl#MisattributedMemory> <https://raw.githubusercontent.com/ranacoskun/cognitive_bias_ontology/main/cbi.owl#CognitiveBias>)

# Class: <https://raw.githubusercontent.com/ranacoskun/cognitive_bias_ontology/main/misattributionOfMemory.owl#OriginalSource> (<https://raw.githubusercontent.com/ranacoskun/cognitive_bias_ontology/main/misattributionOfMemory.owl#OriginalSource>)

AnnotationAssertion(rdfs:comment <https://raw.githubusercontent.com/ranacoskun/cognitive_bias_ontology/main/misattributionOfMemory.owl#OriginalSource> "Describes the Original Source that causes the true instantiation of a memory")
DisjointClasses(<https://raw.githubusercontent.com/ranacoskun/cognitive_bias_ontology/main/misattributionOfMemory.owl#OriginalSource> <https://raw.githubusercontent.com/ranacoskun/cognitive_bias_ontology/main/misattributionOfMemory.owl#SourceConfusion>)

# Class: <https://raw.githubusercontent.com/ranacoskun/cognitive_bias_ontology/main/misattributionOfMemory.owl#Prevention> (<https://raw.githubusercontent.com/ranacoskun/cognitive_bias_ontology/main/misattributionOfMemory.owl#Prevention>)

AnnotationAssertion(rdfs:comment <https://raw.githubusercontent.com/ranacoskun/cognitive_bias_ontology/main/misattributionOfMemory.owl#Prevention> "Strategies or practices aimed at reducing the occurrence of false memories")

# Class: <https://raw.githubusercontent.com/ranacoskun/cognitive_bias_ontology/main/misattributionOfMemory.owl#RecalledIdea> (<https://raw.githubusercontent.com/ranacoskun/cognitive_bias_ontology/main/misattributionOfMemory.owl#RecalledIdea>)

AnnotationAssertion(rdfs:comment <https://raw.githubusercontent.com/ranacoskun/cognitive_bias_ontology/main/misattributionOfMemory.owl#RecalledIdea> "Describes the idea the biased agent thinks they've just created, in this domain refers to a self assessed original creation of any kind, usually a sentence, a joke, a verse.")

# Class: <https://raw.githubusercontent.com/ranacoskun/cognitive_bias_ontology/main/misattributionOfMemory.owl#SourceConfusion> (<https://raw.githubusercontent.com/ranacoskun/cognitive_bias_ontology/main/misattributionOfMemory.owl#SourceConfusion>)

AnnotationAssertion(rdfs:comment <https://raw.githubusercontent.com/ranacoskun/cognitive_bias_ontology/main/misattributionOfMemory.owl#SourceConfusion> "Describes the Source Confusion bias occurrence")
SubClassOf(<https://raw.githubusercontent.com/ranacoskun/cognitive_bias_ontology/main/misattributionOfMemory.owl#SourceConfusion> <https://raw.githubusercontent.com/ranacoskun/cognitive_bias_ontology/main/misattributionOfMemory.owl#MisattributedMemory>)


############################
#   Named Individuals
############################

# Individual: <https://raw.githubusercontent.com/ranacoskun/cognitive_bias_ontology/main/misattributionOfMemory.owl#CCTV_footage> (<https://raw.githubusercontent.com/ranacoskun/cognitive_bias_ontology/main/misattributionOfMemory.owl#CCTV_footage>)

AnnotationAssertion(rdfs:comment <https://raw.githubusercontent.com/ranacoskun/cognitive_bias_ontology/main/misattributionOfMemory.owl#CCTV_footage> "CCTV footage recorded from the bank where the robbery took place.")
ClassAssertion(<https://raw.githubusercontent.com/ranacoskun/cognitive_bias_ontology/main/misattributionOfMemory.owl#Evidence> <https://raw.githubusercontent.com/ranacoskun/cognitive_bias_ontology/main/misattributionOfMemory.owl#CCTV_footage>)

# Individual: <https://raw.githubusercontent.com/ranacoskun/cognitive_bias_ontology/main/misattributionOfMemory.owl#Jane_Doe> (<https://raw.githubusercontent.com/ranacoskun/cognitive_bias_ontology/main/misattributionOfMemory.owl#Jane_Doe>)

AnnotationAssertion(rdfs:comment <https://raw.githubusercontent.com/ranacoskun/cognitive_bias_ontology/main/misattributionOfMemory.owl#Jane_Doe> "A passerby, Jane Doe, claimed to have seen the perpetrator flee the scene.")
ClassAssertion(<https://raw.githubusercontent.com/ranacoskun/cognitive_bias_ontology/main/cbi.owl#BiasedAgent> <https://raw.githubusercontent.com/ranacoskun/cognitive_bias_ontology/main/misattributionOfMemory.owl#Jane_Doe>)

# Individual: <https://raw.githubusercontent.com/ranacoskun/cognitive_bias_ontology/main/misattributionOfMemory.owl#cross_examination_strategy> (<https://raw.githubusercontent.com/ranacoskun/cognitive_bias_ontology/main/misattributionOfMemory.owl#cross_examination_strategy>)

AnnotationAssertion(rdfs:comment <https://raw.githubusercontent.com/ranacoskun/cognitive_bias_ontology/main/misattributionOfMemory.owl#cross_examination_strategy> "Develop a series of questions for Jane Doe that highlight the conditions under which she observed the suspect (e.g., lighting, stress, distance, and her confidence in her recall). Emphasize factors that could have impaired her ability to accurately identify the defendant.")
ClassAssertion(<https://raw.githubusercontent.com/ranacoskun/cognitive_bias_ontology/main/misattributionOfMemory.owl#MemoryTest> <https://raw.githubusercontent.com/ranacoskun/cognitive_bias_ontology/main/misattributionOfMemory.owl#cross_examination_strategy>)

# Individual: <https://raw.githubusercontent.com/ranacoskun/cognitive_bias_ontology/main/misattributionOfMemory.owl#false_accusation> (<https://raw.githubusercontent.com/ranacoskun/cognitive_bias_ontology/main/misattributionOfMemory.owl#false_accusation>)

AnnotationAssertion(rdfs:comment <https://raw.githubusercontent.com/ranacoskun/cognitive_bias_ontology/main/misattributionOfMemory.owl#false_accusation> "The biased agent remembers incorrectly the appearance of a person seen during a robbery.")
ClassAssertion(<https://raw.githubusercontent.com/ranacoskun/cognitive_bias_ontology/main/misattributionOfMemory.owl#FalseMemory> <https://raw.githubusercontent.com/ranacoskun/cognitive_bias_ontology/main/misattributionOfMemory.owl#false_accusation>)

# Individual: <https://raw.githubusercontent.com/ranacoskun/cognitive_bias_ontology/main/misattributionOfMemory.owl#reenactment> (<https://raw.githubusercontent.com/ranacoskun/cognitive_bias_ontology/main/misattributionOfMemory.owl#reenactment>)

AnnotationAssertion(rdfs:comment <https://raw.githubusercontent.com/ranacoskun/cognitive_bias_ontology/main/misattributionOfMemory.owl#reenactment> "Use visual aids or a reenactment to demonstrate to the jury the conditions under which the eyewitness made her observations, including any obstacles, lighting conditions, and the distance from which she viewed the suspect.")
ClassAssertion(<https://raw.githubusercontent.com/ranacoskun/cognitive_bias_ontology/main/misattributionOfMemory.owl#Correction> <https://raw.githubusercontent.com/ranacoskun/cognitive_bias_ontology/main/misattributionOfMemory.owl#reenactment>)

# Individual: <https://raw.githubusercontent.com/ranacoskun/cognitive_bias_ontology/main/misattributionOfMemory.owl#suggestive_questioning> (<https://raw.githubusercontent.com/ranacoskun/cognitive_bias_ontology/main/misattributionOfMemory.owl#suggestive_questioning>)

AnnotationAssertion(rdfs:comment <https://raw.githubusercontent.com/ranacoskun/cognitive_bias_ontology/main/misattributionOfMemory.owl#suggestive_questioning> "A suggestive question is one that implies that a certain answer should be given in response, or falsely presents a presupposition in the question as accepted fact.")
ClassAssertion(<https://raw.githubusercontent.com/ranacoskun/cognitive_bias_ontology/main/misattributionOfMemory.owl#Cause> <https://raw.githubusercontent.com/ranacoskun/cognitive_bias_ontology/main/misattributionOfMemory.owl#suggestive_questioning>)

# Individual: <https://raw.githubusercontent.com/ranacoskun/cognitive_bias_ontology/main/misattributionOfMemory.owl#wrongful_detention> (<https://raw.githubusercontent.com/ranacoskun/cognitive_bias_ontology/main/misattributionOfMemory.owl#wrongful_detention>)

AnnotationAssertion(rdfs:comment <https://raw.githubusercontent.com/ranacoskun/cognitive_bias_ontology/main/misattributionOfMemory.owl#wrongful_detention> "The biased testimony results in the arrest of John Smith")
ClassAssertion(<https://raw.githubusercontent.com/ranacoskun/cognitive_bias_ontology/main/misattributionOfMemory.owl#Effect> <https://raw.githubusercontent.com/ranacoskun/cognitive_bias_ontology/main/misattributionOfMemory.owl#wrongful_detention>)


DisjointClasses(<https://raw.githubusercontent.com/ranacoskun/cognitive_bias_ontology/main/misattributionOfMemory.owl#Cryptomnesia> <https://raw.githubusercontent.com/ranacoskun/cognitive_bias_ontology/main/misattributionOfMemory.owl#FalseMemory> <https://raw.githubusercontent.com/ranacoskun/cognitive_bias_ontology/main/misattributionOfMemory.owl#SourceConfusion>)
)
