<?xml version="1.0"?>
<rdf:RDF xmlns="https://raw.githubusercontent.com/ranacoskun/cognitive_bias_ontology/main/Cue%20Dependent%20Forgetting/Cue-DependentForgetting.owl#"
     xml:base="https://raw.githubusercontent.com/ranacoskun/cognitive_bias_ontology/main/Cue%20Dependent%20Forgetting/Cue-DependentForgetting.owl"
     xmlns:dc="http://purl.org/dc/elements/1.1/"
     xmlns:fs="https://w3id.org/framester/data/framestercore/"
     xmlns:cbi="https://raw.githubusercontent.com/ranacoskun/cognitive_bias_ontology/main/cbi.owl#"
     xmlns:cdf="https://raw.githubusercontent.com/ranacoskun/cognitive_bias_ontology/main/Cue%20Dependent%20Forgetting/Cue-DependentForgetting.owl#"
     xmlns:crm="https://www.cidoc-crm.org/html/cidoc_crm_v7.1.3.html#"
     xmlns:dbo="http://dbpedia.org/ontology/"
     xmlns:owl="http://www.w3.org/2002/07/owl#"
     xmlns:rdf="http://www.w3.org/1999/02/22-rdf-syntax-ns#"
     xmlns:xml="http://www.w3.org/XML/1998/namespace"
     xmlns:xsd="http://www.w3.org/2001/XMLSchema#"
     xmlns:exob="http://ontologydesignpatterns.org/wiki/Submissions:Experience_%26_Observation#"
     xmlns:rdfs="http://www.w3.org/2000/01/rdf-schema#"
     xmlns:reaction="http://www.ontologydesignpatterns.org/cp/owl/reaction.owl.v0.1#"
     xmlns:sequence="http://www.ontologydesignpatterns.org/cp/owl/sequence.owl#"
     xmlns:situation="http://www.ontologydesignpatterns.org/cp/owl/situation.owl#">
    <owl:Ontology rdf:about="https://raw.githubusercontent.com/ranacoskun/cognitive_bias_ontology/main/Cue%20Dependent%20Forgetting/Cue-DependentForgetting.owl">
        <dc:created>13/6/2024</dc:created>
        <dc:creator xml:lang="en">Evgeniia Vdovichenko</dc:creator>
        <dc:description xml:lang="en">Cue-Dependent Forgetting Bias specification of Cognitive Bias Ontology</dc:description>
        <rdfs:comment xml:lang="en">Cue-dependent forgetting bias, also known as retrieval failure, is a phenomenon where the ability to recall information is hindered due to the absence of cues or triggers that were present at the time the memory was encoded. Memory recall is significantly improved by the context or cues that were associated with the initial encoding of the information. These cues can be environmental (such as the place where the learning occurred), emotional (the emotional state at the time of learning), or semantic (related to the meaning of the information).</rdfs:comment>
        <rdfs:label xml:lang="en">Cue-Dependent Forgetting module of the Cognitive Bias Ontology</rdfs:label>
        <owl:versionInfo rdf:datatype="http://www.w3.org/2001/XMLSchema#decimal">2.0</owl:versionInfo>
        <cbi:hasComponent>https://www.cidoc-crm.org/html/cidoc_crm_v7.1.3.html</cbi:hasComponent>
        <cbi:userStory xml:lang="en">It&apos;s the end of the semester, and Alex has been preparing for the final physics exam for weeks. Despite feeling well-prepared the night before, Alex experiences a surge of anxiety as the exam begins, causing a critical formula to slip from memory at a crucial moment. Halfway through the exam, Alex encounters a problem that requires the use of this specific formula. Despite knowing they&apos;ve used it multiple times before, the stress of the exam environment makes it impossible to recall. Frustrated and anxious, Alex moves on to other questions, leaving that part blank.

As time dwindles, Alex reviews their answers, and when revisiting the problematic question, a seemingly unrelated memory flashes through their mind: a joke made by their study group about the formula. This cue, tied to a relaxed and humorous moment, suddenly triggers the forgotten formula&apos;s recall.</cbi:userStory>
    </owl:Ontology>
    


    <!-- 
    ///////////////////////////////////////////////////////////////////////////////////////
    //
    // Annotation properties
    //
    ///////////////////////////////////////////////////////////////////////////////////////
     -->

    


    <!-- http://purl.org/dc/elements/1.1/created -->

    <owl:AnnotationProperty rdf:about="http://purl.org/dc/elements/1.1/created"/>
    


    <!-- http://purl.org/dc/elements/1.1/creator -->

    <owl:AnnotationProperty rdf:about="http://purl.org/dc/elements/1.1/creator"/>
    


    <!-- http://purl.org/dc/elements/1.1/description -->

    <owl:AnnotationProperty rdf:about="http://purl.org/dc/elements/1.1/description"/>
    


    <!-- http://www.w3.org/1999/02/22-rdf-syntax-ns#about -->

    <owl:AnnotationProperty rdf:about="http://www.w3.org/1999/02/22-rdf-syntax-ns#about"/>
    


    <!-- http://www.w3.org/2002/07/owl#versionInfo -->

    <owl:AnnotationProperty rdf:about="http://www.w3.org/2002/07/owl#versionInfo"/>
    


    <!-- https://raw.githubusercontent.com/ranacoskun/cognitive_bias_ontology/main/cbi.owl#hasComponent -->

    <owl:AnnotationProperty rdf:about="https://raw.githubusercontent.com/ranacoskun/cognitive_bias_ontology/main/cbi.owl#hasComponent"/>
    


    <!-- https://raw.githubusercontent.com/ranacoskun/cognitive_bias_ontology/main/cbi.owl#userStory -->

    <owl:AnnotationProperty rdf:about="https://raw.githubusercontent.com/ranacoskun/cognitive_bias_ontology/main/cbi.owl#userStory"/>
    


    <!-- 
    ///////////////////////////////////////////////////////////////////////////////////////
    //
    // Object Properties
    //
    ///////////////////////////////////////////////////////////////////////////////////////
     -->

    


    <!-- http://ontologydesignpatterns.org/wiki/Submissions:Experience_%26_Observation#isEngagedIn -->

    <owl:ObjectProperty rdf:about="http://ontologydesignpatterns.org/wiki/Submissions:Experience_%26_Observation#isEngagedIn">
        <rdfs:domain rdf:resource="https://raw.githubusercontent.com/ranacoskun/cognitive_bias_ontology/main/cbi.owl#BiasedAgent"/>
        <rdfs:range rdf:resource="http://www.ontologydesignpatterns.org/cp/owl/situation.owl#Situation"/>
        <rdfs:comment xml:lang="en">Because an activity may engage other participants than the one performing it, engagements are in general considered individual rather than collective, therefore each participants has their own engagement and only some of them will be conscious and/or documented.</rdfs:comment>
        <rdfs:isDefinedBy>http://ontologydesignpatterns.org/wiki/Submissions:Experience_%26_Observation#isEngagedIn</rdfs:isDefinedBy>
        <rdfs:label xml:lang="en">isEngagedIn</rdfs:label>
    </owl:ObjectProperty>
    


    <!-- http://www.ontologydesignpatterns.org/cp/owl/reaction.owl.v0.1#hasOutcome -->

    <owl:ObjectProperty rdf:about="http://www.ontologydesignpatterns.org/cp/owl/reaction.owl.v0.1#hasOutcome">
        <owl:inverseOf rdf:resource="http://www.ontologydesignpatterns.org/cp/owl/reaction.owl.v0.1#isOutcomeOf"/>
        <rdfs:domain rdf:resource="https://w3id.org/framester/data/framestercore/Memorization"/>
        <rdfs:range rdf:resource="http://dbpedia.org/ontology/Knowledge"/>
        <rdfs:isDefinedBy>http://www.ontologydesignpatterns.org/cp/owl/reaction.owl.v0.1#hasOutcome</rdfs:isDefinedBy>
        <rdfs:label xml:lang="en">hasOutcome</rdfs:label>
        <rdfs:seeAlso>http://ontologydesignpatterns.org/wiki/Submissions:Reaction</rdfs:seeAlso>
    </owl:ObjectProperty>
    


    <!-- http://www.ontologydesignpatterns.org/cp/owl/reaction.owl.v0.1#isOutcomeOf -->

    <owl:ObjectProperty rdf:about="http://www.ontologydesignpatterns.org/cp/owl/reaction.owl.v0.1#isOutcomeOf">
        <rdfs:domain rdf:resource="http://dbpedia.org/ontology/Knowledge"/>
        <rdfs:range rdf:resource="https://w3id.org/framester/data/framestercore/Memorization"/>
        <rdfs:comment xml:lang="en">Is also true that some outcome follows some action</rdfs:comment>
        <rdfs:isDefinedBy>http://www.ontologydesignpatterns.org/cp/owl/reaction.owl.v0.1#isOutcomeOf</rdfs:isDefinedBy>
        <rdfs:label xml:lang="en">isOutcomeOf</rdfs:label>
        <rdfs:seeAlso>http://ontologydesignpatterns.org/wiki/Submissions:Reaction</rdfs:seeAlso>
    </owl:ObjectProperty>
    


    <!-- http://www.ontologydesignpatterns.org/cp/owl/reaction.owl.v0.1#isPerformedBy -->

    <owl:ObjectProperty rdf:about="http://www.ontologydesignpatterns.org/cp/owl/reaction.owl.v0.1#isPerformedBy">
        <owl:inverseOf rdf:resource="http://www.ontologydesignpatterns.org/cp/owl/reaction.owl.v0.1#performs"/>
        <rdfs:domain rdf:resource="https://w3id.org/framester/data/framestercore/Memorization"/>
        <rdfs:range rdf:resource="https://raw.githubusercontent.com/ranacoskun/cognitive_bias_ontology/main/cbi.owl#BiasedAgent"/>
        <rdfs:isDefinedBy>http://www.ontologydesignpatterns.org/cp/owl/reaction.owl.v0.1#isPerformedBy</rdfs:isDefinedBy>
        <rdfs:label xml:lang="en">isPerformedBy</rdfs:label>
        <rdfs:seeAlso>http://ontologydesignpatterns.org/wiki/Submissions:Reaction</rdfs:seeAlso>
    </owl:ObjectProperty>
    


    <!-- http://www.ontologydesignpatterns.org/cp/owl/reaction.owl.v0.1#isRaisedBy -->

    <owl:ObjectProperty rdf:about="http://www.ontologydesignpatterns.org/cp/owl/reaction.owl.v0.1#isRaisedBy">
        <owl:inverseOf rdf:resource="http://www.ontologydesignpatterns.org/cp/owl/reaction.owl.v0.1#raise"/>
        <rdfs:domain rdf:resource="https://raw.githubusercontent.com/ranacoskun/cognitive_bias_ontology/main/Cue%20Dependent%20Forgetting/Cue-DependentForgetting.owl#Reproducing"/>
        <rdfs:range rdf:resource="https://raw.githubusercontent.com/ranacoskun/cognitive_bias_ontology/main/Cue%20Dependent%20Forgetting/Cue-DependentForgetting.owl#Trigger"/>
        <rdfs:isDefinedBy>http://www.ontologydesignpatterns.org/cp/owl/reaction.owl.v0.1#isRaisedBy</rdfs:isDefinedBy>
        <rdfs:label xml:lang="en">isRaisedBy</rdfs:label>
        <rdfs:seeAlso>http://ontologydesignpatterns.org/wiki/Submissions:Reaction</rdfs:seeAlso>
    </owl:ObjectProperty>
    


    <!-- http://www.ontologydesignpatterns.org/cp/owl/reaction.owl.v0.1#performs -->

    <owl:ObjectProperty rdf:about="http://www.ontologydesignpatterns.org/cp/owl/reaction.owl.v0.1#performs">
        <rdfs:domain rdf:resource="https://raw.githubusercontent.com/ranacoskun/cognitive_bias_ontology/main/cbi.owl#BiasedAgent"/>
        <rdfs:range rdf:resource="https://w3id.org/framester/data/framestercore/Memorization"/>
        <rdfs:isDefinedBy>http://www.ontologydesignpatterns.org/cp/owl/reaction.owl.v0.1#performs</rdfs:isDefinedBy>
        <rdfs:label xml:lang="en">performs</rdfs:label>
        <rdfs:seeAlso>http://ontologydesignpatterns.org/wiki/Submissions:Reaction</rdfs:seeAlso>
    </owl:ObjectProperty>
    


    <!-- http://www.ontologydesignpatterns.org/cp/owl/reaction.owl.v0.1#raise -->

    <owl:ObjectProperty rdf:about="http://www.ontologydesignpatterns.org/cp/owl/reaction.owl.v0.1#raise">
        <rdfs:domain rdf:resource="https://raw.githubusercontent.com/ranacoskun/cognitive_bias_ontology/main/Cue%20Dependent%20Forgetting/Cue-DependentForgetting.owl#Trigger"/>
        <rdfs:range rdf:resource="https://raw.githubusercontent.com/ranacoskun/cognitive_bias_ontology/main/Cue%20Dependent%20Forgetting/Cue-DependentForgetting.owl#Reproducing"/>
        <rdfs:isDefinedBy>http://www.ontologydesignpatterns.org/cp/owl/reaction.owl.v0.1#raise</rdfs:isDefinedBy>
        <rdfs:label xml:lang="en">raise</rdfs:label>
        <rdfs:seeAlso>http://ontologydesignpatterns.org/wiki/Submissions:Reaction</rdfs:seeAlso>
    </owl:ObjectProperty>
    


    <!-- http://www.ontologydesignpatterns.org/cp/owl/sequence.owl#precedes -->

    <owl:ObjectProperty rdf:about="http://www.ontologydesignpatterns.org/cp/owl/sequence.owl#precedes">
        <rdfs:domain rdf:resource="https://w3id.org/framester/data/framestercore/Memorization"/>
        <rdfs:range rdf:resource="https://raw.githubusercontent.com/ranacoskun/cognitive_bias_ontology/main/Cue%20Dependent%20Forgetting/Cue-DependentForgetting.owl#Reproducing"/>
        <rdfs:comment xml:lang="en">A relation between entities, expressing a &apos;sequence&apos; schema.</rdfs:comment>
        <rdfs:isDefinedBy>http://www.ontologydesignpatterns.org/cp/owl/sequence.owl#precedes</rdfs:isDefinedBy>
        <rdfs:label xml:lang="en">precedes</rdfs:label>
        <rdfs:seeAlso>http://ontologydesignpatterns.org/wiki/Submissions:Sequence</rdfs:seeAlso>
    </owl:ObjectProperty>
    


    <!-- http://www.ontologydesignpatterns.org/cp/owl/situation.owl#hasSetting -->

    <owl:ObjectProperty rdf:about="http://www.ontologydesignpatterns.org/cp/owl/situation.owl#hasSetting">
        <owl:inverseOf rdf:resource="http://www.ontologydesignpatterns.org/cp/owl/situation.owl#isSettingFor"/>
        <rdfs:domain rdf:resource="https://w3id.org/framester/data/framestercore/Memorization"/>
        <rdfs:range rdf:resource="http://www.ontologydesignpatterns.org/cp/owl/situation.owl#Situation"/>
        <rdfs:comment xml:lang="en">A relation between entities and situations, e.g. this morning I&apos;ve prepared my coffee with a new fantastic Arabica; (i.e.: (an amount of) a new fantastic Arabica hasSetting the preparation of my coffee this morning).</rdfs:comment>
        <rdfs:isDefinedBy>http://www.ontologydesignpatterns.org/cp/owl/situation.owl#hasSetting</rdfs:isDefinedBy>
        <rdfs:label xml:lang="en">hasSetting</rdfs:label>
        <rdfs:seeAlso>http://ontologydesignpatterns.org/wiki/Submissions:Situation</rdfs:seeAlso>
    </owl:ObjectProperty>
    


    <!-- http://www.ontologydesignpatterns.org/cp/owl/situation.owl#isSettingFor -->

    <owl:ObjectProperty rdf:about="http://www.ontologydesignpatterns.org/cp/owl/situation.owl#isSettingFor">
        <rdfs:domain rdf:resource="http://www.ontologydesignpatterns.org/cp/owl/situation.owl#Situation"/>
        <rdfs:range rdf:resource="https://w3id.org/framester/data/framestercore/Memorization"/>
        <rdfs:isDefinedBy>http://www.ontologydesignpatterns.org/cp/owl/situation.owl#hasSetting</rdfs:isDefinedBy>
        <rdfs:label xml:lang="en">isSettingFor</rdfs:label>
        <rdfs:seeAlso>http://ontologydesignpatterns.org/wiki/Submissions:Situation</rdfs:seeAlso>
    </owl:ObjectProperty>
    


    <!-- https://raw.githubusercontent.com/ranacoskun/cognitive_bias_ontology/main/cbi.owl#affectedBy -->

    <owl:ObjectProperty rdf:about="https://raw.githubusercontent.com/ranacoskun/cognitive_bias_ontology/main/cbi.owl#affectedBy">
        <owl:inverseOf rdf:resource="https://raw.githubusercontent.com/ranacoskun/cognitive_bias_ontology/main/cbi.owl#affects"/>
        <rdf:type rdf:resource="http://www.w3.org/2002/07/owl#TransitiveProperty"/>
        <rdfs:domain rdf:resource="https://raw.githubusercontent.com/ranacoskun/cognitive_bias_ontology/main/cbi.owl#BiasedAgent"/>
        <rdfs:range rdf:resource="https://raw.githubusercontent.com/ranacoskun/cognitive_bias_ontology/main/cbi.owl#CognitiveBias"/>
        <rdfs:comment xml:lang="en">Describes the relationship between a Cognitive Bias and an Individual on the base of influence.</rdfs:comment>
        <rdfs:isDefinedBy>https://raw.githubusercontent.com/ranacoskun/cognitive_bias_ontology/main/cbi.owl#affectedBy</rdfs:isDefinedBy>
        <rdfs:label xml:lang="en">affectedBy</rdfs:label>
    </owl:ObjectProperty>
    


    <!-- https://raw.githubusercontent.com/ranacoskun/cognitive_bias_ontology/main/cbi.owl#affects -->

    <owl:ObjectProperty rdf:about="https://raw.githubusercontent.com/ranacoskun/cognitive_bias_ontology/main/cbi.owl#affects">
        <rdf:type rdf:resource="http://www.w3.org/2002/07/owl#TransitiveProperty"/>
        <rdfs:domain rdf:resource="https://raw.githubusercontent.com/ranacoskun/cognitive_bias_ontology/main/cbi.owl#CognitiveBias"/>
        <rdfs:range rdf:resource="https://raw.githubusercontent.com/ranacoskun/cognitive_bias_ontology/main/cbi.owl#BiasedAgent"/>
        <rdfs:comment xml:lang="en">Inverse of AffectedBy.</rdfs:comment>
        <rdfs:isDefinedBy>https://raw.githubusercontent.com/ranacoskun/cognitive_bias_ontology/main/cbi.owl#affects</rdfs:isDefinedBy>
        <rdfs:label xml:lang="en">affects</rdfs:label>
    </owl:ObjectProperty>
    


    <!-- https://raw.githubusercontent.com/ranacoskun/cognitive_bias_ontology/main/cbi.owl#hasTrigger -->

    <owl:ObjectProperty rdf:about="https://raw.githubusercontent.com/ranacoskun/cognitive_bias_ontology/main/cbi.owl#hasTrigger">
        <rdfs:domain rdf:resource="http://www.ontologydesignpatterns.org/cp/owl/situation.owl#Situation"/>
        <rdfs:range rdf:resource="https://raw.githubusercontent.com/ranacoskun/cognitive_bias_ontology/main/Cue%20Dependent%20Forgetting/Cue-DependentForgetting.owl#Trigger"/>
        <rdfs:comment xml:lang="en">Signifies the stimuli, conditions, or events that initiate or activate a specific cognitive process.</rdfs:comment>
        <rdfs:isDefinedBy>https://raw.githubusercontent.com/ranacoskun/cognitive_bias_ontology/main/cbi.owl#hasTrigger</rdfs:isDefinedBy>
        <rdfs:label xml:lang="en">hasTrigger</rdfs:label>
    </owl:ObjectProperty>
    


    <!-- https://www.cidoc-crm.org/html/cidoc_crm_v7.1.3.html#isAbout -->

    <owl:ObjectProperty rdf:about="https://www.cidoc-crm.org/html/cidoc_crm_v7.1.3.html#isAbout">
        <rdfs:domain rdf:resource="http://dbpedia.org/ontology/Knowledge"/>
        <rdfs:range rdf:resource="https://w3id.org/framester/data/framestercore/Information"/>
        <rdfs:comment xml:lang="en">This property documents that an instance of E89 Propositional Object has as subject an instance of E1 CRM Entity. This differs from P67 refers to (is referred to by), which refers to an instance of E1 CRM Entity, in that it describes the primary subject or subjects of an instance of E89 Propositional Object.</rdfs:comment>
        <rdfs:isDefinedBy>https://www.cidoc-crm.org/html/cidoc_crm_v7.1.3.html#isAbout</rdfs:isDefinedBy>
        <rdfs:label xml:lang="en">isAbout</rdfs:label>
        <rdfs:seeAlso>https://cidoc-crm.org/html/cidoc_crm_v7.1.3.html#P129</rdfs:seeAlso>
    </owl:ObjectProperty>
    


    <!-- https://www.cidoc-crm.org/html/cidoc_crm_v7.1.3.html#usedSpecificObject -->

    <owl:ObjectProperty rdf:about="https://www.cidoc-crm.org/html/cidoc_crm_v7.1.3.html#usedSpecificObject">
        <rdfs:domain rdf:resource="https://raw.githubusercontent.com/ranacoskun/cognitive_bias_ontology/main/Cue%20Dependent%20Forgetting/Cue-DependentForgetting.owl#Reproducing"/>
        <rdfs:domain rdf:resource="https://w3id.org/framester/data/framestercore/Memorization"/>
        <rdfs:range rdf:resource="http://dbpedia.org/ontology/Knowledge"/>
        <rdfs:range rdf:resource="https://w3id.org/framester/data/framestercore/Information"/>
        <rdfs:comment xml:lang="en">This property describes the use of material or immaterial things in a way essential to the performance or the outcome of an instance of E7 Activity. It implies that the presence of the object in question was a necessary condition for the action.</rdfs:comment>
        <rdfs:isDefinedBy>https://www.cidoc-crm.org/html/cidoc_crm_v7.1.3.html#usedSpecificObject</rdfs:isDefinedBy>
        <rdfs:label xml:lang="en">used specific object</rdfs:label>
        <rdfs:seeAlso>https://cidoc-crm.org/html/cidoc_crm_v7.1.3.html#P16</rdfs:seeAlso>
    </owl:ObjectProperty>
    


    <!-- 
    ///////////////////////////////////////////////////////////////////////////////////////
    //
    // Data properties
    //
    ///////////////////////////////////////////////////////////////////////////////////////
     -->

    


    <!-- https://www.cidoc-crm.org/html/cidoc_crm_v7.1.3.html#hasType -->

    <owl:DatatypeProperty rdf:about="https://www.cidoc-crm.org/html/cidoc_crm_v7.1.3.html#hasType">
        <rdf:type rdf:resource="http://www.w3.org/2002/07/owl#FunctionalProperty"/>
        <rdfs:domain rdf:resource="https://raw.githubusercontent.com/ranacoskun/cognitive_bias_ontology/main/Cue%20Dependent%20Forgetting/Cue-DependentForgetting.owl#Trigger"/>
        <rdfs:range rdf:resource="http://www.w3.org/2001/XMLSchema#string"/>
        <rdfs:comment xml:lang="en">This property allows sub-typing of entities – a form of specialization – through the use of a terminological hierarchy, or thesaurus.</rdfs:comment>
        <rdfs:isDefinedBy>https://www.cidoc-crm.org/html/cidoc_crm_v7.1.3.html#hasType</rdfs:isDefinedBy>
        <rdfs:label xml:lang="en">hasType</rdfs:label>
        <rdfs:seeAlso rdf:resource="https://cidoc-crm.org/html/cidoc_crm_v7.1.3.html#P2"/>
    </owl:DatatypeProperty>
    


    <!-- 
    ///////////////////////////////////////////////////////////////////////////////////////
    //
    // Classes
    //
    ///////////////////////////////////////////////////////////////////////////////////////
     -->

    


    <!-- http://dbpedia.org/ontology/Knowledge -->

    <owl:Class rdf:about="http://dbpedia.org/ontology/Knowledge">
        <rdfs:comment xml:lang="en">Can be defined as awareness of facts or as practical skills and may also refer to familiarity with objects or situations. Knowledge of facts, also called propositional knowledge, is often defined as true belief that is distinct from opinion or guesswork by virtue of justification. While there is wide agreement among philosophers that propositional knowledge is a form of true belief, many controversies in philosophy focus on justification: whether it is needed at all, how to understand it, and whether something else besides it is needed. These controversies intensified due to a series of thought experiments by Edmund Gettier and have provoked various alternative definitions. Some of them deny that justification is necessary and replace it, for example, with reliability or the man.</rdfs:comment>
        <rdfs:isDefinedBy>http://dbpedia.org/ontology/Knowledge</rdfs:isDefinedBy>
        <rdfs:label xml:lang="en">Knowledge</rdfs:label>
    </owl:Class>
    


    <!-- http://www.ontologydesignpatterns.org/cp/owl/situation.owl#Situation -->

    <owl:Class rdf:about="http://www.ontologydesignpatterns.org/cp/owl/situation.owl#Situation">
        <rdfs:comment xml:lang="en">A view on a set of entities. It can be seen as a relational context, reifying a relation.
For example, a PlanExecution is a context including some actions executed by agents according to certain parameters and expected tasks to be achieved from a Plan; a DiagnosedSituation is a context of observed entities that is interpreted on the basis of a Diagnosis, etc.

Situation is also able to represent reified n-ary relations, where isSettingFor is the top-level relation for all binary projections of the n-ary relation. If used in a transformation pattern for n-ary relations, the designer should take care of:

- creating only one situation for each instance of an n-ary relation, otherwise the identification constraint (Calvanese et al., IJCAI 2001) could be violated

- adding an exact cardinality restriction corresponding to the arity of the n-ary relation, otherwise the designer would actually represent a polymorphic relation.</rdfs:comment>
        <rdfs:isDefinedBy>http://www.ontologydesignpatterns.org/cp/owl/situation.owl#Situation</rdfs:isDefinedBy>
        <rdfs:label xml:lang="en">Situation</rdfs:label>
    </owl:Class>
    


    <!-- https://raw.githubusercontent.com/ranacoskun/cognitive_bias_ontology/main/Cue%20Dependent%20Forgetting/Cue-DependentForgetting.owl#Reproducing -->

    <owl:Class rdf:about="https://raw.githubusercontent.com/ranacoskun/cognitive_bias_ontology/main/Cue%20Dependent%20Forgetting/Cue-DependentForgetting.owl#Reproducing">
        <owl:equivalentClass>
            <owl:Restriction>
                <owl:onProperty rdf:resource="https://www.cidoc-crm.org/html/cidoc_crm_v7.1.3.html#usedSpecificObject"/>
                <owl:allValuesFrom rdf:resource="http://dbpedia.org/ontology/Knowledge"/>
            </owl:Restriction>
        </owl:equivalentClass>
        <rdfs:comment xml:lang="en">Models the process of recalling and possibly reconstructing memories. This class deals with how an agent processes and reproduces information from memory.</rdfs:comment>
        <rdfs:isDefinedBy>https://raw.githubusercontent.com/ranacoskun/cognitive_bias_ontology/main/Cue%20Dependent%20Forgetting/Cue-DependentForgetting.owl#Reproducing</rdfs:isDefinedBy>
        <rdfs:label xml:lang="en">Reproducing</rdfs:label>
    </owl:Class>
    


    <!-- https://raw.githubusercontent.com/ranacoskun/cognitive_bias_ontology/main/Cue%20Dependent%20Forgetting/Cue-DependentForgetting.owl#Trigger -->

    <owl:Class rdf:about="https://raw.githubusercontent.com/ranacoskun/cognitive_bias_ontology/main/Cue%20Dependent%20Forgetting/Cue-DependentForgetting.owl#Trigger">
        <owl:equivalentClass>
            <owl:Class>
                <owl:unionOf rdf:parseType="Collection">
                    <owl:Restriction>
                        <owl:onProperty rdf:resource="https://www.cidoc-crm.org/html/cidoc_crm_v7.1.3.html#hasType"/>
                        <owl:hasValue>context-dependent</owl:hasValue>
                    </owl:Restriction>
                    <owl:Restriction>
                        <owl:onProperty rdf:resource="https://www.cidoc-crm.org/html/cidoc_crm_v7.1.3.html#hasType"/>
                        <owl:hasValue>state-dependent</owl:hasValue>
                    </owl:Restriction>
                </owl:unionOf>
            </owl:Class>
        </owl:equivalentClass>
        <rdfs:comment xml:lang="en">Represents an environmental or contextual stimulus that facilitates the recall of memories by a BiasedAgent. Has types depending on the provenance of the trigger: context-dependent (referring to the environment) and state-dependent (referring to the person experiencing the bias).</rdfs:comment>
        <rdfs:isDefinedBy>https://raw.githubusercontent.com/ranacoskun/cognitive_bias_ontology/main/cbi.owl#Trigger</rdfs:isDefinedBy>
        <rdfs:label xml:lang="en">Trigger</rdfs:label>
    </owl:Class>
    


    <!-- https://raw.githubusercontent.com/ranacoskun/cognitive_bias_ontology/main/cbi.owl#BiasedAgent -->

    <owl:Class rdf:about="https://raw.githubusercontent.com/ranacoskun/cognitive_bias_ontology/main/cbi.owl#BiasedAgent">
        <rdfs:subClassOf rdf:resource="https://w3id.org/framester/data/framestercore/People"/>
        <rdfs:comment xml:lang="en">Represents an entity that experiences the bias.</rdfs:comment>
        <rdfs:isDefinedBy>https://raw.githubusercontent.com/ranacoskun/cognitive_bias_ontology/main/cbi.owl#BiasedAgent</rdfs:isDefinedBy>
        <rdfs:label xml:lang="en">BiasedAgent</rdfs:label>
    </owl:Class>
    


    <!-- https://raw.githubusercontent.com/ranacoskun/cognitive_bias_ontology/main/cbi.owl#CognitiveBias -->

    <owl:Class rdf:about="https://raw.githubusercontent.com/ranacoskun/cognitive_bias_ontology/main/cbi.owl#CognitiveBias">
        <rdfs:comment xml:lang="en">Represents the overarching concept of cognitive biases.</rdfs:comment>
        <rdfs:isDefinedBy>https://raw.githubusercontent.com/ranacoskun/cognitive_bias_ontology/main/cbi.owl#CognitiveBias</rdfs:isDefinedBy>
        <rdfs:label xml:lang="en">CognitiveBias</rdfs:label>
    </owl:Class>
    


    <!-- https://raw.githubusercontent.com/ranacoskun/cognitive_bias_ontology/main/cbi.owl#CueDependentForgetting -->

    <owl:Class rdf:about="https://raw.githubusercontent.com/ranacoskun/cognitive_bias_ontology/main/cbi.owl#CueDependentForgetting">
        <rdfs:subClassOf rdf:resource="https://raw.githubusercontent.com/ranacoskun/cognitive_bias_ontology/main/cbi.owl#CognitiveBias"/>
        <rdfs:comment xml:lang="en">A specific cognitive bias where the ability to recall information is dependent on cues present at the time of encoding and at the time of retrieval.</rdfs:comment>
        <rdfs:isDefinedBy>https://raw.githubusercontent.com/ranacoskun/cognitive_bias_ontology/main/cbi.owl#CueDependentForgetting</rdfs:isDefinedBy>
        <rdfs:label xml:lang="en">CueDependentForgetting</rdfs:label>
    </owl:Class>
    


    <!-- https://w3id.org/framester/data/framestercore/Information -->

    <owl:Class rdf:about="https://w3id.org/framester/data/framestercore/Information">
        <rdfs:comment xml:lang="en">Describes the information which the person would like to memorize.</rdfs:comment>
        <rdfs:isDefinedBy>https://w3id.org/framester/data/framestercore/Information</rdfs:isDefinedBy>
        <rdfs:label xml:lang="en">Information</rdfs:label>
    </owl:Class>
    


    <!-- https://w3id.org/framester/data/framestercore/Memorization -->

    <owl:Class rdf:about="https://w3id.org/framester/data/framestercore/Memorization">
        <owl:equivalentClass>
            <owl:Restriction>
                <owl:onProperty rdf:resource="https://www.cidoc-crm.org/html/cidoc_crm_v7.1.3.html#usedSpecificObject"/>
                <owl:allValuesFrom rdf:resource="https://w3id.org/framester/data/framestercore/Information"/>
            </owl:Restriction>
        </owl:equivalentClass>
        <rdfs:comment xml:lang="en">Models memorizing activity.</rdfs:comment>
        <rdfs:isDefinedBy>https://w3id.org/framester/data/framestercore/Memorization</rdfs:isDefinedBy>
        <rdfs:label xml:lang="en">Memorization</rdfs:label>
    </owl:Class>
    


    <!-- https://w3id.org/framester/data/framestercore/People -->

    <owl:Class rdf:about="https://w3id.org/framester/data/framestercore/People">
        <rdfs:comment xml:lang="en">Denotes a human being and express that we are talking about human cognitive biases.</rdfs:comment>
        <rdfs:isDefinedBy>https://w3id.org/framester/data/framestercore/People</rdfs:isDefinedBy>
        <rdfs:label xml:lang="en">People</rdfs:label>
    </owl:Class>
    


    <!-- 
    ///////////////////////////////////////////////////////////////////////////////////////
    //
    // Individuals
    //
    ///////////////////////////////////////////////////////////////////////////////////////
     -->

    


    <!-- https://raw.githubusercontent.com/ranacoskun/cognitive_bias_ontology/main/Cue%20Dependent%20Forgetting/Cue-DependentForgetting.owl#Alex -->

    <owl:NamedIndividual rdf:about="https://raw.githubusercontent.com/ranacoskun/cognitive_bias_ontology/main/Cue%20Dependent%20Forgetting/Cue-DependentForgetting.owl#Alex">
        <rdf:type rdf:resource="https://raw.githubusercontent.com/ranacoskun/cognitive_bias_ontology/main/cbi.owl#BiasedAgent"/>
        <exob:isEngagedIn rdf:resource="https://raw.githubusercontent.com/ranacoskun/cognitive_bias_ontology/main/Cue%20Dependent%20Forgetting/Cue-DependentForgetting.owl#Exam"/>
        <reaction:performs rdf:resource="https://raw.githubusercontent.com/ranacoskun/cognitive_bias_ontology/main/Cue%20Dependent%20Forgetting/Cue-DependentForgetting.owl#FormulaKnowledge"/>
        <reaction:performs rdf:resource="https://raw.githubusercontent.com/ranacoskun/cognitive_bias_ontology/main/Cue%20Dependent%20Forgetting/Cue-DependentForgetting.owl#FormulaUsage"/>
        <cbi:affectedBy rdf:resource="https://raw.githubusercontent.com/ranacoskun/cognitive_bias_ontology/main/Cue%20Dependent%20Forgetting/Cue-DependentForgetting.owl#CueDependentForgettingInstance"/>
        <rdfs:comment xml:lang="en">Alex is a student who experiences the Cue-Dependent Forgetting Bias.</rdfs:comment>
        <rdfs:isDefinedBy>https://raw.githubusercontent.com/ranacoskun/cognitive_bias_ontology/main/Cue%20Dependent%20Forgetting/Cue-DependentForgetting.owl#Alex</rdfs:isDefinedBy>
        <rdfs:label xml:lang="en">Alex</rdfs:label>
    </owl:NamedIndividual>
    


    <!-- https://raw.githubusercontent.com/ranacoskun/cognitive_bias_ontology/main/Cue%20Dependent%20Forgetting/Cue-DependentForgetting.owl#CueDependentForgettingInstance -->

    <owl:NamedIndividual rdf:about="https://raw.githubusercontent.com/ranacoskun/cognitive_bias_ontology/main/Cue%20Dependent%20Forgetting/Cue-DependentForgetting.owl#CueDependentForgettingInstance">
        <rdf:type rdf:resource="https://raw.githubusercontent.com/ranacoskun/cognitive_bias_ontology/main/cbi.owl#CueDependentForgetting"/>
        <rdfs:comment xml:lang="en">The situation of expiriencing the Cue-Dependent Forgetting Bias</rdfs:comment>
        <rdfs:isDefinedBy>https://raw.githubusercontent.com/ranacoskun/cognitive_bias_ontology/main/Cue%20Dependent%20Forgetting/Cue-DependentForgetting.owl#CueDependentForgettingInstance</rdfs:isDefinedBy>
        <rdfs:label xml:lang="en">Cue-Dependent Forgetting Instance</rdfs:label>
    </owl:NamedIndividual>
    


    <!-- https://raw.githubusercontent.com/ranacoskun/cognitive_bias_ontology/main/Cue%20Dependent%20Forgetting/Cue-DependentForgetting.owl#Exam -->

    <owl:NamedIndividual rdf:about="https://raw.githubusercontent.com/ranacoskun/cognitive_bias_ontology/main/Cue%20Dependent%20Forgetting/Cue-DependentForgetting.owl#Exam">
        <rdf:type rdf:resource="http://www.ontologydesignpatterns.org/cp/owl/situation.owl#Situation"/>
        <situation:hasSetting rdf:resource="https://raw.githubusercontent.com/ranacoskun/cognitive_bias_ontology/main/Cue%20Dependent%20Forgetting/Cue-DependentForgetting.owl#ExamPreparation"/>
        <cbi:hasTrigger rdf:resource="https://raw.githubusercontent.com/ranacoskun/cognitive_bias_ontology/main/Cue%20Dependent%20Forgetting/Cue-DependentForgetting.owl#Joke"/>
        <rdfs:comment xml:lang="en">This is the final physics exam that Alex is taking, which triggers a surge of anxiety and leads to a memory failure.</rdfs:comment>
        <rdfs:isDefinedBy>https://raw.githubusercontent.com/ranacoskun/cognitive_bias_ontology/main/Cue%20Dependent%20Forgetting/Cue-DependentForgetting.owl#Exam</rdfs:isDefinedBy>
        <rdfs:label xml:lang="en">Exam</rdfs:label>
    </owl:NamedIndividual>
    


    <!-- https://raw.githubusercontent.com/ranacoskun/cognitive_bias_ontology/main/Cue%20Dependent%20Forgetting/Cue-DependentForgetting.owl#ExamPreparation -->

    <owl:NamedIndividual rdf:about="https://raw.githubusercontent.com/ranacoskun/cognitive_bias_ontology/main/Cue%20Dependent%20Forgetting/Cue-DependentForgetting.owl#ExamPreparation">
        <rdf:type rdf:resource="https://w3id.org/framester/data/framestercore/Memorization"/>
        <reaction:hasOutcome rdf:resource="https://raw.githubusercontent.com/ranacoskun/cognitive_bias_ontology/main/Cue%20Dependent%20Forgetting/Cue-DependentForgetting.owl#FormulaKnowledge"/>
        <sequence:precedes rdf:resource="https://raw.githubusercontent.com/ranacoskun/cognitive_bias_ontology/main/Cue%20Dependent%20Forgetting/Cue-DependentForgetting.owl#FormulaUsage"/>
        <situation:isSettingFor rdf:resource="https://raw.githubusercontent.com/ranacoskun/cognitive_bias_ontology/main/Cue%20Dependent%20Forgetting/Cue-DependentForgetting.owl#Exam"/>
        <crm:usedSpecificObject rdf:resource="https://raw.githubusercontent.com/ranacoskun/cognitive_bias_ontology/main/Cue%20Dependent%20Forgetting/Cue-DependentForgetting.owl#Formula"/>
        <rdfs:comment xml:lang="en">Preparing for the final physics exam.</rdfs:comment>
        <rdfs:isDefinedBy>https://raw.githubusercontent.com/ranacoskun/cognitive_bias_ontology/main/Cue%20Dependent%20Forgetting/Cue-DependentForgetting.owl#ExamPreparation</rdfs:isDefinedBy>
        <rdfs:label xml:lang="en">Exam Preparation</rdfs:label>
    </owl:NamedIndividual>
    


    <!-- https://raw.githubusercontent.com/ranacoskun/cognitive_bias_ontology/main/Cue%20Dependent%20Forgetting/Cue-DependentForgetting.owl#Formula -->

    <owl:NamedIndividual rdf:about="https://raw.githubusercontent.com/ranacoskun/cognitive_bias_ontology/main/Cue%20Dependent%20Forgetting/Cue-DependentForgetting.owl#Formula">
        <rdf:type rdf:resource="https://w3id.org/framester/data/framestercore/Information"/>
        <rdfs:comment xml:lang="en">A critical formula which Alex need for exam.</rdfs:comment>
        <rdfs:isDefinedBy>https://raw.githubusercontent.com/ranacoskun/cognitive_bias_ontology/main/Cue%20Dependent%20Forgetting/Cue-DependentForgetting.owl#Formula</rdfs:isDefinedBy>
        <rdfs:label xml:lang="en">Formula</rdfs:label>
    </owl:NamedIndividual>
    


    <!-- https://raw.githubusercontent.com/ranacoskun/cognitive_bias_ontology/main/Cue%20Dependent%20Forgetting/Cue-DependentForgetting.owl#FormulaKnowledge -->

    <owl:NamedIndividual rdf:about="https://raw.githubusercontent.com/ranacoskun/cognitive_bias_ontology/main/Cue%20Dependent%20Forgetting/Cue-DependentForgetting.owl#FormulaKnowledge">
        <rdf:type rdf:resource="http://dbpedia.org/ontology/Knowledge"/>
        <reaction:isOutcomeOf rdf:resource="https://raw.githubusercontent.com/ranacoskun/cognitive_bias_ontology/main/Cue%20Dependent%20Forgetting/Cue-DependentForgetting.owl#ExamPreparation"/>
        <crm:isAbout rdf:resource="https://raw.githubusercontent.com/ranacoskun/cognitive_bias_ontology/main/Cue%20Dependent%20Forgetting/Cue-DependentForgetting.owl#Formula"/>
        <rdfs:comment xml:lang="en">The knowledge of the specific formula</rdfs:comment>
        <rdfs:isDefinedBy>https://raw.githubusercontent.com/ranacoskun/cognitive_bias_ontology/main/Cue%20Dependent%20Forgetting/Cue-DependentForgetting.owl#FormulaKnowledge</rdfs:isDefinedBy>
        <rdfs:label xml:lang="en">Formula Knowledge</rdfs:label>
    </owl:NamedIndividual>
    


    <!-- https://raw.githubusercontent.com/ranacoskun/cognitive_bias_ontology/main/Cue%20Dependent%20Forgetting/Cue-DependentForgetting.owl#FormulaUsage -->

    <owl:NamedIndividual rdf:about="https://raw.githubusercontent.com/ranacoskun/cognitive_bias_ontology/main/Cue%20Dependent%20Forgetting/Cue-DependentForgetting.owl#FormulaUsage">
        <rdf:type rdf:resource="https://raw.githubusercontent.com/ranacoskun/cognitive_bias_ontology/main/Cue%20Dependent%20Forgetting/Cue-DependentForgetting.owl#Reproducing"/>
        <reaction:isPerformedBy rdf:resource="https://raw.githubusercontent.com/ranacoskun/cognitive_bias_ontology/main/Cue%20Dependent%20Forgetting/Cue-DependentForgetting.owl#Alex"/>
        <reaction:isRaisedBy rdf:resource="https://raw.githubusercontent.com/ranacoskun/cognitive_bias_ontology/main/Cue%20Dependent%20Forgetting/Cue-DependentForgetting.owl#Joke"/>
        <crm:usedSpecificObject rdf:resource="https://raw.githubusercontent.com/ranacoskun/cognitive_bias_ontology/main/Cue%20Dependent%20Forgetting/Cue-DependentForgetting.owl#FormulaKnowledge"/>
        <rdfs:comment xml:lang="en">Using of the specific formula during the exam.</rdfs:comment>
        <rdfs:isDefinedBy>https://raw.githubusercontent.com/ranacoskun/cognitive_bias_ontology/main/Cue%20Dependent%20Forgetting/Cue-DependentForgetting.owl#FormulaUsage</rdfs:isDefinedBy>
        <rdfs:label xml:lang="en">Formula Usage</rdfs:label>
    </owl:NamedIndividual>
    


    <!-- https://raw.githubusercontent.com/ranacoskun/cognitive_bias_ontology/main/Cue%20Dependent%20Forgetting/Cue-DependentForgetting.owl#Joke -->

    <owl:NamedIndividual rdf:about="https://raw.githubusercontent.com/ranacoskun/cognitive_bias_ontology/main/Cue%20Dependent%20Forgetting/Cue-DependentForgetting.owl#Joke">
        <rdf:type rdf:resource="https://raw.githubusercontent.com/ranacoskun/cognitive_bias_ontology/main/Cue%20Dependent%20Forgetting/Cue-DependentForgetting.owl#Trigger"/>
        <reaction:raise rdf:resource="https://raw.githubusercontent.com/ranacoskun/cognitive_bias_ontology/main/Cue%20Dependent%20Forgetting/Cue-DependentForgetting.owl#FormulaUsage"/>
        <crm:hasType>context-dependent</crm:hasType>
        <rdfs:comment xml:lang="en">A joke made by the study group, which triggers the recall of the forgotten formula.</rdfs:comment>
        <rdfs:isDefinedBy xml:lang="en">https://raw.githubusercontent.com/ranacoskun/cognitive_bias_ontology/main/Cue%20Dependent%20Forgetting/Cue-DependentForgetting.owl#Joke</rdfs:isDefinedBy>
        <rdfs:label xml:lang="en">Joke</rdfs:label>
    </owl:NamedIndividual>
</rdf:RDF>



<!-- Generated by the OWL API (version 4.5.26.2023-07-17T20:34:13Z) https://github.com/owlcs/owlapi -->

