<?xml version="1.0"?>
<rdf:RDF xmlns="https://raw.githubusercontent.com/ranacoskun/cognitive_bias_ontology/main/Baader-Meinhof%20Phenomenon/Baader-Meinhof%20Phenomenon.owl#"
     xml:base="https://raw.githubusercontent.com/ranacoskun/cognitive_bias_ontology/main/Baader-Meinhof%20Phenomenon/Baader-Meinhof%20Phenomenon.owl"
     xmlns:dc="http://purl.org/dc/elements/1.1/"
     xmlns:fs="https://w3id.org/framester/data/framestercore/"
     xmlns:bmp="https://raw.githubusercontent.com/ranacoskun/cognitive_bias_ontology/main/Baader-Meinhof%20Phenomenon/Baader-Meinhof%20Phenomenon.owl#"
     xmlns:cbi="https://raw.githubusercontent.com/ranacoskun/cognitive_bias_ontology/main/cbi.owl#"
     xmlns:cco="http://smiy.sourceforge.net/cco/spec/cognitivecharacteristics.html#"
     xmlns:crm="https://www.cidoc-crm.org/html/cidoc_crm_v7.1.3.html#"
     xmlns:dbo="http://dbpedia.org/ontology/"
     xmlns:owl="http://www.w3.org/2002/07/owl#"
     xmlns:rdf="http://www.w3.org/1999/02/22-rdf-syntax-ns#"
     xmlns:xml="http://www.w3.org/XML/1998/namespace"
     xmlns:xsd="http://www.w3.org/2001/XMLSchema#"
     xmlns:exob="http://ontologydesignpatterns.org/wiki/Submissions:Experience_%26_Observation#"
     xmlns:fsyn="https://w3id.org/framester/data/framestersyn/"
     xmlns:rdfs="http://www.w3.org/2000/01/rdf-schema#"
     xmlns:skos="https://www.w3.org/TR/skos-reference/"
     xmlns:reaction="http://www.ontologydesignpatterns.org/cp/owl/reaction.owl.v0.1#"
     xmlns:sequence="http://www.ontologydesignpatterns.org/cp/owl/sequence.owl#"
     xmlns:parameter="http://www.ontologydesignpatterns.org/cp/owl/parameter.owl#"
     xmlns:situation="http://www.ontologydesignpatterns.org/cp/owl/situation.owl#">
    <owl:Ontology rdf:about="https://raw.githubusercontent.com/ranacoskun/cognitive_bias_ontology/main/Baader-Meinhof%20Phenomenon/Baader-Meinhof%20Phenomenon.owl">
        <dc:created>13/6/2024</dc:created>
        <dc:creator xml:lang="en">Evgeniia Vdovichenko</dc:creator>
        <dc:description xml:lang="en">Baader-Meinhof Phenomenon specification of Cognitive Bias Ontology</dc:description>
        <rdfs:comment xml:lang="en">The Baader-Meinhof phenomenon, also known as the Frequency Illusion, is a cognitive bias in which after noticing something for the first time, there is a tendency to notice it more frequently thereafter, leading one to believe that it has an increased frequency of occurrence. This perception is not due to the actual increase in frequency but rather due to the new awareness of the item, event, or term.

In essence, while the Baader-Meinhof Phenomenon often refers to more distinctive or unusual observations, the frequency illusion can apply to any information, whether common or rare. Both terms describe the same underlying cognitive bias of increased awareness and selective attention, but the Baader-Meinhof Phenomenon has a flavor of novelty and rarity attached to it.</rdfs:comment>
        <rdfs:isDefinedBy xml:lang="en">https://raw.githubusercontent.com/ranacoskun/cognitive_bias_ontology/main/Baader-Meinhof%20Phenomenon/Baader-Meinhof%20Phenomenon.owl</rdfs:isDefinedBy>
        <rdfs:label xml:lang="en">Baader-Meinhof Phenomenon module of the Cognitive Bias Ontology</rdfs:label>
        <owl:versionInfo rdf:datatype="http://www.w3.org/2001/XMLSchema#decimal">2.0</owl:versionInfo>
        <cbi:hasComponent>http://dbpedia.org/ontology/</cbi:hasComponent>
        <cbi:hasComponent>http://ontologydesignpatterns.org/wiki/Submissions:Experience_%26_Observation</cbi:hasComponent>
        <cbi:hasComponent>http://www.ontologydesignpatterns.org/cp/owl/parameter.owl</cbi:hasComponent>
        <cbi:hasComponent>http://www.ontologydesignpatterns.org/cp/owl/reaction.owl.v0.1</cbi:hasComponent>
        <cbi:hasComponent>http://www.ontologydesignpatterns.org/cp/owl/sequence.owl</cbi:hasComponent>
        <cbi:hasComponent>http://www.ontologydesignpatterns.org/cp/owl/situation.owl</cbi:hasComponent>
        <cbi:hasComponent>https://w3id.org/framester/data/framestercore/</cbi:hasComponent>
        <cbi:hasComponent>https://w3id.org/framester/data/framestersyn/</cbi:hasComponent>
        <cbi:hasComponent>https://www.cidoc-crm.org/html/cidoc_crm_v7.1.3.html</cbi:hasComponent>
        <cbi:hasComponent>https://www.w3.org/TR/skos-reference/</cbi:hasComponent>
        <cbi:hasComponent>smiy.sourceforge.net/cco/spec/cognitivecharacteristics.html</cbi:hasComponent>
        <cbi:userStory xml:lang="en">After learning the word &apos;solipsism&apos; in a philosophy class, Jamie began to encounter it everywhere: in a psychology book, during a podcast, and even in a news article about perception. This amusing frequency of a once unfamiliar term led Jamie to appreciate how new knowledge can suddenly resonate across different mediums, enhancing awareness and deepening their engagement with ongoing learning.</cbi:userStory>
    </owl:Ontology>
    


    <!-- 
    ///////////////////////////////////////////////////////////////////////////////////////
    //
    // Annotation properties
    //
    ///////////////////////////////////////////////////////////////////////////////////////
     -->

    


    <!-- http://purl.org/dc/elements/1.1/created -->

    <owl:AnnotationProperty rdf:about="http://purl.org/dc/elements/1.1/created"/>
    


    <!-- http://purl.org/dc/elements/1.1/creator -->

    <owl:AnnotationProperty rdf:about="http://purl.org/dc/elements/1.1/creator"/>
    


    <!-- http://purl.org/dc/elements/1.1/description -->

    <owl:AnnotationProperty rdf:about="http://purl.org/dc/elements/1.1/description"/>
    


    <!-- http://www.w3.org/1999/02/22-rdf-syntax-ns#about -->

    <owl:AnnotationProperty rdf:about="http://www.w3.org/1999/02/22-rdf-syntax-ns#about"/>
    


    <!-- http://www.w3.org/2002/07/owl#versionInfo -->

    <owl:AnnotationProperty rdf:about="http://www.w3.org/2002/07/owl#versionInfo"/>
    


    <!-- https://raw.githubusercontent.com/ranacoskun/cognitive_bias_ontology/main/cbi.owl#hasComponent -->

    <owl:AnnotationProperty rdf:about="https://raw.githubusercontent.com/ranacoskun/cognitive_bias_ontology/main/cbi.owl#hasComponent"/>
    


    <!-- https://raw.githubusercontent.com/ranacoskun/cognitive_bias_ontology/main/cbi.owl#userStory -->

    <owl:AnnotationProperty rdf:about="https://raw.githubusercontent.com/ranacoskun/cognitive_bias_ontology/main/cbi.owl#userStory"/>
    


    <!-- 
    ///////////////////////////////////////////////////////////////////////////////////////
    //
    // Object Properties
    //
    ///////////////////////////////////////////////////////////////////////////////////////
     -->

    


    <!-- http://ontologydesignpatterns.org/wiki/Submissions:Experience_%26_Observation#isEngagedIn -->

    <owl:ObjectProperty rdf:about="http://ontologydesignpatterns.org/wiki/Submissions:Experience_%26_Observation#isEngagedIn">
        <rdfs:domain rdf:resource="https://raw.githubusercontent.com/ranacoskun/cognitive_bias_ontology/main/cbi.owl#BiasedAgent"/>
        <rdfs:range rdf:resource="https://w3id.org/framester/data/framestercore/BecomingAware"/>
        <rdfs:range rdf:resource="https://w3id.org/framester/data/framestercore/PerceptionExperience"/>
        <rdfs:comment xml:lang="en">Because an activity may engage other participants than the one performing it, engagements are in general considered individual rather than collective, therefore each participants has their own engagement and only some of them will be conscious and/or documented.</rdfs:comment>
        <rdfs:isDefinedBy>http://ontologydesignpatterns.org/wiki/Submissions:Experience_%26_Observation#isEngagedIn</rdfs:isDefinedBy>
        <rdfs:label xml:lang="en">isEngagedIn</rdfs:label>
    </owl:ObjectProperty>
    


    <!-- http://smiy.sourceforge.net/cco/spec/cognitivecharacteristics.html#belief -->

    <owl:ObjectProperty rdf:about="http://smiy.sourceforge.net/cco/spec/cognitivecharacteristics.html#belief">
        <rdfs:domain rdf:resource="https://raw.githubusercontent.com/ranacoskun/cognitive_bias_ontology/main/cbi.owl#BiasedAgent"/>
        <rdfs:range rdf:resource="https://w3id.org/framester/data/framestersyn/Belief"/>
        <rdfs:comment xml:lang="en">Property which means that a person has belief - an uncertain relation for competence representation. That means beliefs, persuasions or opinions, which can also be misconceptions.</rdfs:comment>
        <rdfs:isDefinedBy>http://smiy.sourceforge.net/cco/spec/cognitivecharacteristics.html#belief</rdfs:isDefinedBy>
        <rdfs:label xml:lang="en">belief</rdfs:label>
    </owl:ObjectProperty>
    


    <!-- http://www.ontologydesignpatterns.org/cp/owl/parameter.owl#hasParameter -->

    <owl:ObjectProperty rdf:about="http://www.ontologydesignpatterns.org/cp/owl/parameter.owl#hasParameter">
        <owl:inverseOf rdf:resource="http://www.ontologydesignpatterns.org/cp/owl/parameter.owl#isParameterFor"/>
        <rdfs:domain rdf:resource="https://w3id.org/framester/data/framestercore/PerceptionExperience"/>
        <rdfs:range rdf:resource="https://w3id.org/framester/data/framestercore/Frequency"/>
        <rdfs:comment xml:lang="en">A Concept can have a Parameter that constrains the attributes that a classified Entity can have in a certain Situation, e.g. a 4WheelDriver Role definedIn the ItalianTrafficLaw has a MinimumAge parameter on the Amount 16.</rdfs:comment>
        <rdfs:isDefinedBy>http://www.ontologydesignpatterns.org/cp/owl/parameter.owl#hasParameter</rdfs:isDefinedBy>
        <rdfs:label xml:lang="en">hasParameter</rdfs:label>
        <rdfs:seeAlso>http://ontologydesignpatterns.org/wiki/Submissions:Parameter</rdfs:seeAlso>
    </owl:ObjectProperty>
    


    <!-- http://www.ontologydesignpatterns.org/cp/owl/parameter.owl#isParameterFor -->

    <owl:ObjectProperty rdf:about="http://www.ontologydesignpatterns.org/cp/owl/parameter.owl#isParameterFor">
        <rdfs:domain rdf:resource="https://w3id.org/framester/data/framestercore/Frequency"/>
        <rdfs:range rdf:resource="https://w3id.org/framester/data/framestercore/PerceptionExperience"/>
        <rdfs:comment xml:lang="en">A Concept can have a Parameter that constrains the attributes that a classified Entity can have in a certain Situation, e.g. a 4WheelDriver Role definedIn the ItalianTrafficLaw has a MinimumAge parameter on the Amount 16</rdfs:comment>
        <rdfs:isDefinedBy>http://www.ontologydesignpatterns.org/cp/owl/parameter.owl#isParameterFor</rdfs:isDefinedBy>
        <rdfs:label xml:lang="en">isParameterFor</rdfs:label>
        <rdfs:seeAlso>http://ontologydesignpatterns.org/wiki/Submissions:Parameter</rdfs:seeAlso>
    </owl:ObjectProperty>
    


    <!-- http://www.ontologydesignpatterns.org/cp/owl/reaction.owl.v0.1#hasOutcome -->

    <owl:ObjectProperty rdf:about="http://www.ontologydesignpatterns.org/cp/owl/reaction.owl.v0.1#hasOutcome">
        <owl:inverseOf rdf:resource="http://www.ontologydesignpatterns.org/cp/owl/reaction.owl.v0.1#isOutcomeOf"/>
        <rdfs:domain rdf:resource="https://w3id.org/framester/data/framestercore/BecomingAware"/>
        <rdfs:range rdf:resource="http://dbpedia.org/ontology/Knowledge"/>
        <rdfs:comment xml:lang="en">Is also true that some action directly preceeds its outcome</rdfs:comment>
        <rdfs:isDefinedBy>http://www.ontologydesignpatterns.org/cp/owl/reaction.owl.v0.1#hasOutcome</rdfs:isDefinedBy>
        <rdfs:label xml:lang="en">hasOutcome</rdfs:label>
        <rdfs:seeAlso>http://ontologydesignpatterns.org/wiki/Submissions:Reaction</rdfs:seeAlso>
    </owl:ObjectProperty>
    


    <!-- http://www.ontologydesignpatterns.org/cp/owl/reaction.owl.v0.1#isOutcomeOf -->

    <owl:ObjectProperty rdf:about="http://www.ontologydesignpatterns.org/cp/owl/reaction.owl.v0.1#isOutcomeOf">
        <rdfs:domain rdf:resource="http://dbpedia.org/ontology/Knowledge"/>
        <rdfs:range rdf:resource="https://w3id.org/framester/data/framestercore/BecomingAware"/>
        <rdfs:comment xml:lang="en">Is also true that some outcome follows some action</rdfs:comment>
        <rdfs:isDefinedBy>http://www.ontologydesignpatterns.org/cp/owl/reaction.owl.v0.1#isOutcomeOf</rdfs:isDefinedBy>
        <rdfs:label xml:lang="en">isOutcomeOf</rdfs:label>
        <rdfs:seeAlso>http://ontologydesignpatterns.org/wiki/Submissions:Reaction</rdfs:seeAlso>
    </owl:ObjectProperty>
    


    <!-- http://www.ontologydesignpatterns.org/cp/owl/sequence.owl#precedes -->

    <owl:ObjectProperty rdf:about="http://www.ontologydesignpatterns.org/cp/owl/sequence.owl#precedes">
        <rdfs:domain rdf:resource="https://w3id.org/framester/data/framestercore/BecomingAware"/>
        <rdfs:range rdf:resource="https://w3id.org/framester/data/framestercore/PerceptionExperience"/>
        <rdfs:comment xml:lang="en">A relation between entities, expressing a sequence schema.</rdfs:comment>
        <rdfs:isDefinedBy>http://www.ontologydesignpatterns.org/cp/owl/sequence.owl#precedes</rdfs:isDefinedBy>
        <rdfs:label xml:lang="en">precedes</rdfs:label>
        <rdfs:seeAlso>http://ontologydesignpatterns.org/wiki/Submissions:Sequence</rdfs:seeAlso>
    </owl:ObjectProperty>
    


    <!-- http://www.ontologydesignpatterns.org/cp/owl/situation.owl#hasSetting -->

    <owl:ObjectProperty rdf:about="http://www.ontologydesignpatterns.org/cp/owl/situation.owl#hasSetting">
        <owl:inverseOf rdf:resource="http://www.ontologydesignpatterns.org/cp/owl/situation.owl#isSettingFor"/>
        <rdfs:domain rdf:resource="https://w3id.org/framester/data/framestercore/PerceptionExperience"/>
        <rdfs:range rdf:resource="http://dbpedia.org/ontology/Concept"/>
        <rdfs:comment xml:lang="en">A relation between entities and situations, e.g. this morning I&apos;ve prepared my coffee with a new fantastic Arabica&amp;apos; (i.e.: (an amount of) a new fantastic Arabica hasSetting the preparation of my coffee this morning).</rdfs:comment>
        <rdfs:isDefinedBy>http://www.ontologydesignpatterns.org/cp/owl/situation.owl#hasSetting</rdfs:isDefinedBy>
        <rdfs:label xml:lang="en">hasSetting</rdfs:label>
        <rdfs:seeAlso>http://ontologydesignpatterns.org/wiki/Submissions:Situation</rdfs:seeAlso>
    </owl:ObjectProperty>
    


    <!-- http://www.ontologydesignpatterns.org/cp/owl/situation.owl#isSettingFor -->

    <owl:ObjectProperty rdf:about="http://www.ontologydesignpatterns.org/cp/owl/situation.owl#isSettingFor">
        <rdfs:domain rdf:resource="http://dbpedia.org/ontology/Concept"/>
        <rdfs:range rdf:resource="https://w3id.org/framester/data/framestercore/PerceptionExperience"/>
        <rdfs:isDefinedBy>http://www.ontologydesignpatterns.org/cp/owl/situation.owl#isSettingFor</rdfs:isDefinedBy>
        <rdfs:label xml:lang="en">isSettingFor</rdfs:label>
        <rdfs:seeAlso>http://ontologydesignpatterns.org/wiki/Submissions:Situation</rdfs:seeAlso>
    </owl:ObjectProperty>
    


    <!-- http://www.w3.org/2004/02/skos/core#related -->

    <owl:ObjectProperty rdf:about="http://www.w3.org/2004/02/skos/core#related">
        <rdf:type rdf:resource="http://www.w3.org/2002/07/owl#SymmetricProperty"/>
        <rdfs:domain rdf:resource="https://raw.githubusercontent.com/ranacoskun/cognitive_bias_ontology/main/cbi.owl#Baader-MeinhofPhenomenon"/>
        <rdfs:range rdf:resource="https://raw.githubusercontent.com/ranacoskun/cognitive_bias_ontology/main/cbi.owl#FrequencyIllusion"/>
        <rdfs:comment xml:lang="en">Property which asserts an associative link between two concepts.</rdfs:comment>
        <rdfs:isDefinedBy>http://www.w3.org/2004/02/skos/core#related</rdfs:isDefinedBy>
        <rdfs:isDefinedBy>https://www.w3.org/2009/08/skos-reference/skos.html#related</rdfs:isDefinedBy>
        <rdfs:label>related</rdfs:label>
    </owl:ObjectProperty>
    


    <!-- https://raw.githubusercontent.com/ranacoskun/cognitive_bias_ontology/main/cbi.owl#affectedBy -->

    <owl:ObjectProperty rdf:about="https://raw.githubusercontent.com/ranacoskun/cognitive_bias_ontology/main/cbi.owl#affectedBy">
        <owl:inverseOf rdf:resource="https://raw.githubusercontent.com/ranacoskun/cognitive_bias_ontology/main/cbi.owl#affects"/>
        <rdf:type rdf:resource="http://www.w3.org/2002/07/owl#TransitiveProperty"/>
        <rdfs:domain rdf:resource="https://raw.githubusercontent.com/ranacoskun/cognitive_bias_ontology/main/cbi.owl#BiasedAgent"/>
        <rdfs:range rdf:resource="https://raw.githubusercontent.com/ranacoskun/cognitive_bias_ontology/main/cbi.owl#CognitiveBias"/>
        <rdfs:comment xml:lang="en">Describes the relationship between a Cognitive Bias and an Individual on the base of influence.</rdfs:comment>
        <rdfs:isDefinedBy>https://raw.githubusercontent.com/ranacoskun/cognitive_bias_ontology/main/cbi.owl#affectedBy</rdfs:isDefinedBy>
        <rdfs:label xml:lang="en">affectedBy</rdfs:label>
    </owl:ObjectProperty>
    


    <!-- https://raw.githubusercontent.com/ranacoskun/cognitive_bias_ontology/main/cbi.owl#affects -->

    <owl:ObjectProperty rdf:about="https://raw.githubusercontent.com/ranacoskun/cognitive_bias_ontology/main/cbi.owl#affects">
        <rdf:type rdf:resource="http://www.w3.org/2002/07/owl#TransitiveProperty"/>
        <rdfs:domain rdf:resource="https://raw.githubusercontent.com/ranacoskun/cognitive_bias_ontology/main/cbi.owl#CognitiveBias"/>
        <rdfs:range rdf:resource="https://raw.githubusercontent.com/ranacoskun/cognitive_bias_ontology/main/cbi.owl#BiasedAgent"/>
        <rdfs:comment xml:lang="en">Inverse of AffectedBy.</rdfs:comment>
        <rdfs:isDefinedBy>https://raw.githubusercontent.com/ranacoskun/cognitive_bias_ontology/main/cbi.owl#affects</rdfs:isDefinedBy>
        <rdfs:label xml:lang="en">affects</rdfs:label>
    </owl:ObjectProperty>
    


    <!-- https://raw.githubusercontent.com/ranacoskun/cognitive_bias_ontology/main/cbi.owl#influences -->

    <owl:ObjectProperty rdf:about="https://raw.githubusercontent.com/ranacoskun/cognitive_bias_ontology/main/cbi.owl#influences">
        <rdfs:domain rdf:resource="https://w3id.org/framester/data/framestercore/PerceptionExperience"/>
        <rdfs:range rdf:resource="https://w3id.org/framester/data/framestersyn/Belief"/>
        <rdfs:comment xml:lang="en">An entity having and effect on the other entity</rdfs:comment>
        <rdfs:isDefinedBy>https://raw.githubusercontent.com/ranacoskun/cognitive_bias_ontology/main/cbi.owl#influences</rdfs:isDefinedBy>
        <rdfs:label xml:lang="en">influences</rdfs:label>
    </owl:ObjectProperty>
    


    <!-- https://www.cidoc-crm.org/html/cidoc_crm_v7.1.3.html#isAbout -->

    <owl:ObjectProperty rdf:about="https://www.cidoc-crm.org/html/cidoc_crm_v7.1.3.html#isAbout">
        <rdfs:domain rdf:resource="http://dbpedia.org/ontology/Knowledge"/>
        <rdfs:domain rdf:resource="https://w3id.org/framester/data/framestersyn/Belief"/>
        <rdfs:range rdf:resource="http://dbpedia.org/ontology/Concept"/>
        <rdfs:range rdf:resource="https://w3id.org/framester/data/framestercore/Frequency"/>
        <rdfs:comment xml:lang="en">This property documents that an instance of E89 Propositional Object has as subject an instance of E1 CRM Entity. This differs from P67 refers to (is referred to by), which refers to an instance of E1 CRM Entity, in that it describes the primary subject or subjects of an instance of E89 Propositional Object.</rdfs:comment>
        <rdfs:isDefinedBy>https://cidoc-crm.org/html/cidoc_crm_v7.1.3.html#P129</rdfs:isDefinedBy>
        <rdfs:label xml:lang="en">isAbout</rdfs:label>
    </owl:ObjectProperty>
    


    <!-- 
    ///////////////////////////////////////////////////////////////////////////////////////
    //
    // Data properties
    //
    ///////////////////////////////////////////////////////////////////////////////////////
     -->

    


    <!-- http://www.ontologydesignpatterns.org/cp/owl/parameter.owl#hasParameterDataValue -->

    <owl:DatatypeProperty rdf:about="http://www.ontologydesignpatterns.org/cp/owl/parameter.owl#hasParameterDataValue">
        <rdf:type rdf:resource="http://www.w3.org/2002/07/owl#FunctionalProperty"/>
        <rdfs:domain rdf:resource="https://w3id.org/framester/data/framestercore/Frequency"/>
        <rdfs:range rdf:resource="http://www.w3.org/2001/XMLSchema#string"/>
        <rdfs:isDefinedBy>http://www.ontologydesignpatterns.org/cp/owl/parameter.owl#hasParameterDataValue</rdfs:isDefinedBy>
        <rdfs:label xml:lang="en">hasParameterDataValue</rdfs:label>
        <rdfs:seeAlso rdf:resource="http://ontologydesignpatterns.org/wiki/Submissions:Parameter"/>
    </owl:DatatypeProperty>
    


    <!-- 
    ///////////////////////////////////////////////////////////////////////////////////////
    //
    // Classes
    //
    ///////////////////////////////////////////////////////////////////////////////////////
     -->

    


    <!-- http://dbpedia.org/ontology/Concept -->

    <owl:Class rdf:about="http://dbpedia.org/ontology/Concept">
        <rdfs:comment xml:lang="en">Concepts are defined as abstract ideas. They are understood to be the fundamental building blocks of the concept behind principles, thoughts and beliefs.They play an important role in all aspects of cognition. As such, concepts are studied by several disciplines, such as linguistics, psychology, and philosophy, and these disciplines are interested in the logical and psychological structure of concepts, and how they are put together to form thoughts and sentences. The study of concepts has served as an important flagship of an emerging interdisciplinary approach called cognitive science.</rdfs:comment>
        <rdfs:isDefinedBy>https://dbpedia.org/page/Concept</rdfs:isDefinedBy>
        <rdfs:label xml:lang="en">Concept</rdfs:label>
    </owl:Class>
    


    <!-- http://dbpedia.org/ontology/Knowledge -->

    <owl:Class rdf:about="http://dbpedia.org/ontology/Knowledge">
        <owl:equivalentClass>
            <owl:Restriction>
                <owl:onProperty rdf:resource="https://www.cidoc-crm.org/html/cidoc_crm_v7.1.3.html#isAbout"/>
                <owl:allValuesFrom rdf:resource="http://dbpedia.org/ontology/Concept"/>
            </owl:Restriction>
        </owl:equivalentClass>
        <rdfs:comment xml:lang="en">Can be defined as awareness of facts or as practical skills and may also refer to familiarity with objects or situations. Knowledge of facts, also called propositional knowledge, is often defined as true belief that is distinct from opinion or guesswork by virtue of justification. While there is wide agreement among philosophers that propositional knowledge is a form of true belief, many controversies in philosophy focus on justification: whether it is needed at all, how to understand it, and whether something else besides it is needed. These controversies intensified due to a series of thought experiments by Edmund Gettier and have provoked various alternative definitions. Some of them deny that justification is necessary and replace it, for example, with reliability or the man.</rdfs:comment>
        <rdfs:isDefinedBy>https://dbpedia.org/page/Knowledge</rdfs:isDefinedBy>
        <rdfs:label xml:lang="en">Knowledge</rdfs:label>
    </owl:Class>
    


    <!-- https://raw.githubusercontent.com/ranacoskun/cognitive_bias_ontology/main/cbi.owl#Baader-MeinhofPhenomenon -->

    <owl:Class rdf:about="https://raw.githubusercontent.com/ranacoskun/cognitive_bias_ontology/main/cbi.owl#Baader-MeinhofPhenomenon">
        <rdfs:subClassOf rdf:resource="https://raw.githubusercontent.com/ranacoskun/cognitive_bias_ontology/main/cbi.owl#CognitiveBias"/>
        <rdfs:comment xml:lang="en">Represents another type of the cognitive bias - Baader-MeinhofPhenomenon - a cognitive bias wherein after noticing something for the first time, there is a tendency to notice it more often, leading someone to believe that it has an increased frequency of occurrence. This is not due to the actual increase in frequency but rather due to the individual&amp;apos;s selective attention and heightened awareness. Some sources call it also Frequency Illusion.</rdfs:comment>
        <rdfs:isDefinedBy>https://raw.githubusercontent.com/ranacoskun/cognitive_bias_ontology/main/cbi.owl#Baader-MeinhofPhenomenon</rdfs:isDefinedBy>
        <rdfs:label xml:lang="en">Baader-MeinhofPhenomenon</rdfs:label>
    </owl:Class>
    


    <!-- https://raw.githubusercontent.com/ranacoskun/cognitive_bias_ontology/main/cbi.owl#BiasedAgent -->

    <owl:Class rdf:about="https://raw.githubusercontent.com/ranacoskun/cognitive_bias_ontology/main/cbi.owl#BiasedAgent">
        <owl:equivalentClass>
            <owl:Restriction>
                <owl:onProperty rdf:resource="http://ontologydesignpatterns.org/wiki/Submissions:Experience_%26_Observation#isEngagedIn"/>
                <owl:someValuesFrom rdf:resource="https://w3id.org/framester/data/framestercore/BecomingAware"/>
            </owl:Restriction>
        </owl:equivalentClass>
        <owl:equivalentClass>
            <owl:Restriction>
                <owl:onProperty rdf:resource="http://ontologydesignpatterns.org/wiki/Submissions:Experience_%26_Observation#isEngagedIn"/>
                <owl:someValuesFrom rdf:resource="https://w3id.org/framester/data/framestercore/PerceptionExperience"/>
            </owl:Restriction>
        </owl:equivalentClass>
        <rdfs:subClassOf rdf:resource="https://w3id.org/framester/data/framestercore/People"/>
        <rdfs:comment xml:lang="en">Represents an entity that experiences the bias.</rdfs:comment>
        <rdfs:isDefinedBy>https://raw.githubusercontent.com/ranacoskun/cognitive_bias_ontology/main/cbi.owl#BiasedAgent</rdfs:isDefinedBy>
        <rdfs:label xml:lang="en">BiasedAgent</rdfs:label>
    </owl:Class>
    


    <!-- https://raw.githubusercontent.com/ranacoskun/cognitive_bias_ontology/main/cbi.owl#CognitiveBias -->

    <owl:Class rdf:about="https://raw.githubusercontent.com/ranacoskun/cognitive_bias_ontology/main/cbi.owl#CognitiveBias">
        <rdfs:comment xml:lang="en">Represents the overarching concept of cognitive biases.</rdfs:comment>
        <rdfs:isDefinedBy>https://raw.githubusercontent.com/ranacoskun/cognitive_bias_ontology/main/cbi.owl#CognitiveBias</rdfs:isDefinedBy>
        <rdfs:label xml:lang="en">CognitiveBias</rdfs:label>
    </owl:Class>
    


    <!-- https://raw.githubusercontent.com/ranacoskun/cognitive_bias_ontology/main/cbi.owl#FrequencyIllusion -->

    <owl:Class rdf:about="https://raw.githubusercontent.com/ranacoskun/cognitive_bias_ontology/main/cbi.owl#FrequencyIllusion">
        <rdfs:subClassOf rdf:resource="https://raw.githubusercontent.com/ranacoskun/cognitive_bias_ontology/main/cbi.owl#CognitiveBias"/>
        <rdfs:comment xml:lang="en">A cognitive bias where a person believes a recently noticed item or concept has suddenly become prevalent.</rdfs:comment>
        <rdfs:isDefinedBy>https://raw.githubusercontent.com/ranacoskun/cognitive_bias_ontology/main/cbi.owl#FrequencyIllusion</rdfs:isDefinedBy>
        <rdfs:label xml:lang="en">FrequencyIllusion</rdfs:label>
    </owl:Class>
    


    <!-- https://w3id.org/framester/data/framestercore/BecomingAware -->

    <owl:Class rdf:about="https://w3id.org/framester/data/framestercore/BecomingAware">
        <rdfs:comment xml:lang="en">The process of learning new things and concepts.</rdfs:comment>
        <rdfs:isDefinedBy>https://w3id.org/framester/data/framestercore/BecomingAware</rdfs:isDefinedBy>
        <rdfs:label xml:lang="en">BecomingAware</rdfs:label>
    </owl:Class>
    


    <!-- https://w3id.org/framester/data/framestercore/Frequency -->

    <owl:Class rdf:about="https://w3id.org/framester/data/framestercore/Frequency">
        <owl:equivalentClass>
            <owl:Restriction>
                <owl:onProperty rdf:resource="http://www.ontologydesignpatterns.org/cp/owl/parameter.owl#hasParameterDataValue"/>
                <owl:hasValue>high</owl:hasValue>
            </owl:Restriction>
        </owl:equivalentClass>
        <rdfs:comment xml:lang="en">Represents the frequency of perception experience of a particular concept, which seem to happen more often under the influence of bias.</rdfs:comment>
        <rdfs:isDefinedBy>https://w3id.org/framester/data/framestercore/Frequency</rdfs:isDefinedBy>
        <rdfs:label xml:lang="en">Frequency</rdfs:label>
    </owl:Class>
    


    <!-- https://w3id.org/framester/data/framestercore/People -->

    <owl:Class rdf:about="https://w3id.org/framester/data/framestercore/People">
        <rdfs:comment xml:lang="en">Used to denote a human being and express that we are talking about human cognitive biases.</rdfs:comment>
        <rdfs:isDefinedBy>https://w3id.org/framester/data/framestercore/People</rdfs:isDefinedBy>
        <rdfs:label xml:lang="en">People</rdfs:label>
    </owl:Class>
    


    <!-- https://w3id.org/framester/data/framestercore/PerceptionExperience -->

    <owl:Class rdf:about="https://w3id.org/framester/data/framestercore/PerceptionExperience">
        <rdfs:comment xml:lang="en">Models the activity of perception of the concept.</rdfs:comment>
        <rdfs:isDefinedBy>https://w3id.org/framester/data/framestercore/PerceptionExperience</rdfs:isDefinedBy>
        <rdfs:label xml:lang="en">PerceptionExperience</rdfs:label>
    </owl:Class>
    


    <!-- https://w3id.org/framester/data/framestersyn/Belief -->

    <owl:Class rdf:about="https://w3id.org/framester/data/framestersyn/Belief">
        <owl:equivalentClass>
            <owl:Restriction>
                <owl:onProperty rdf:resource="https://www.cidoc-crm.org/html/cidoc_crm_v7.1.3.html#isAbout"/>
                <owl:allValuesFrom rdf:resource="https://w3id.org/framester/data/framestercore/Frequency"/>
            </owl:Restriction>
        </owl:equivalentClass>
        <rdfs:comment xml:lang="en">A belief is a mental state or attitude where an individual holds something to be true or probable. Beliefs can range from factual assertions about the world to subjective evaluations, opinions, or attitudes about various matters. Beliefs can be based on evidence, personal experience, cultural upbringing, social influences, or even intuition. 

Неre we used it to show that the BiasedAgent has the biased opinion (belief) to express that it is only opinion but not the real state of things.</rdfs:comment>
        <rdfs:isDefinedBy>http://etna.istc.cnr.it/framesterpage/data/framestersyn/Belief.n.1</rdfs:isDefinedBy>
        <rdfs:label xml:lang="en">Belief</rdfs:label>
    </owl:Class>
    


    <!-- 
    ///////////////////////////////////////////////////////////////////////////////////////
    //
    // Individuals
    //
    ///////////////////////////////////////////////////////////////////////////////////////
     -->

    


    <!-- https://raw.githubusercontent.com/ranacoskun/cognitive_bias_ontology/main/Baader-Meinhof%20Phenomenon/Baader-Meinhof%20Phenomenon.owl#Baader-MeinhofPhenomenonInstance -->

    <owl:NamedIndividual rdf:about="https://raw.githubusercontent.com/ranacoskun/cognitive_bias_ontology/main/Baader-Meinhof%20Phenomenon/Baader-Meinhof%20Phenomenon.owl#Baader-MeinhofPhenomenonInstance">
        <rdf:type rdf:resource="https://raw.githubusercontent.com/ranacoskun/cognitive_bias_ontology/main/cbi.owl#Baader-MeinhofPhenomenon"/>
        <cbi:affects rdf:resource="https://raw.githubusercontent.com/ranacoskun/cognitive_bias_ontology/main/cbi.owl#Jamie"/>
        <rdfs:comment xml:lang="en">The situation of expiriencing the Baader-Meinhof Phenomenon.</rdfs:comment>
        <rdfs:isDefinedBy>https://raw.githubusercontent.com/ranacoskun/cognitive_bias_ontology/main/Baader-Meinhof%20Phenomenon/Baader-Meinhof%20Phenomenon.owl#Baader-MeinhofPhenomenonInstance</rdfs:isDefinedBy>
        <rdfs:label xml:lang="en">Baader-Meinhof Phenomenon Instance</rdfs:label>
    </owl:NamedIndividual>
    


    <!-- https://raw.githubusercontent.com/ranacoskun/cognitive_bias_ontology/main/Baader-Meinhof%20Phenomenon/Baader-Meinhof%20Phenomenon.owl#FrequencyBelief -->

    <owl:NamedIndividual rdf:about="https://raw.githubusercontent.com/ranacoskun/cognitive_bias_ontology/main/Baader-Meinhof%20Phenomenon/Baader-Meinhof%20Phenomenon.owl#FrequencyBelief">
        <rdf:type rdf:resource="https://w3id.org/framester/data/framestersyn/Belief"/>
        <crm:isAbout rdf:resource="https://raw.githubusercontent.com/ranacoskun/cognitive_bias_ontology/main/Baader-Meinhof%20Phenomenon/Baader-Meinhof%20Phenomenon.owl#FrequencyOfSolipsism"/>
        <rdfs:comment xml:lang="en">The belief that the increased frequency of encountering the term &quot;solipsism&quot; is due to an actual increase in its occurrence, rather than increased awareness.</rdfs:comment>
        <rdfs:isDefinedBy>https://raw.githubusercontent.com/ranacoskun/cognitive_bias_ontology/main/Baader-Meinhof%20Phenomenon/Baader-Meinhof%20Phenomenon.owl#FrequencyBelief</rdfs:isDefinedBy>
        <rdfs:label xml:lang="en">Frequency Belief</rdfs:label>
    </owl:NamedIndividual>
    


    <!-- https://raw.githubusercontent.com/ranacoskun/cognitive_bias_ontology/main/Baader-Meinhof%20Phenomenon/Baader-Meinhof%20Phenomenon.owl#FrequencyOfSolipsism -->

    <owl:NamedIndividual rdf:about="https://raw.githubusercontent.com/ranacoskun/cognitive_bias_ontology/main/Baader-Meinhof%20Phenomenon/Baader-Meinhof%20Phenomenon.owl#FrequencyOfSolipsism">
        <rdf:type rdf:resource="https://w3id.org/framester/data/framestercore/Frequency"/>
        <parameter:isParameterFor rdf:resource="https://raw.githubusercontent.com/ranacoskun/cognitive_bias_ontology/main/Baader-Meinhof%20Phenomenon/Baader-Meinhof%20Phenomenon.owl#RecognisingSolipsism"/>
        <parameter:hasParameterDataValue>high</parameter:hasParameterDataValue>
        <rdfs:comment xml:lang="en">The observed increase in the frequency of encountering the term &quot;solipsism&quot; in various contexts after initially learning about it.</rdfs:comment>
        <rdfs:isDefinedBy>https://raw.githubusercontent.com/ranacoskun/cognitive_bias_ontology/main/Baader-Meinhof%20Phenomenon/Baader-Meinhof%20Phenomenon.owl#FrequencyOfSolipsism</rdfs:isDefinedBy>
        <rdfs:label xml:lang="en">Solipsism Frequency</rdfs:label>
    </owl:NamedIndividual>
    


    <!-- https://raw.githubusercontent.com/ranacoskun/cognitive_bias_ontology/main/Baader-Meinhof%20Phenomenon/Baader-Meinhof%20Phenomenon.owl#LearningSolipsism -->

    <owl:NamedIndividual rdf:about="https://raw.githubusercontent.com/ranacoskun/cognitive_bias_ontology/main/Baader-Meinhof%20Phenomenon/Baader-Meinhof%20Phenomenon.owl#LearningSolipsism">
        <rdf:type rdf:resource="https://w3id.org/framester/data/framestercore/BecomingAware"/>
        <reaction:hasOutcome rdf:resource="https://raw.githubusercontent.com/ranacoskun/cognitive_bias_ontology/main/Baader-Meinhof%20Phenomenon/Baader-Meinhof%20Phenomenon.owl#SolipsismKnowledge"/>
        <sequence:precedes rdf:resource="https://raw.githubusercontent.com/ranacoskun/cognitive_bias_ontology/main/Baader-Meinhof%20Phenomenon/Baader-Meinhof%20Phenomenon.owl#RecognisingSolipsism"/>
        <rdfs:comment xml:lang="en">Learning about  the concept &quot;solipsism&quot;.</rdfs:comment>
        <rdfs:isDefinedBy>https://raw.githubusercontent.com/ranacoskun/cognitive_bias_ontology/main/Baader-Meinhof%20Phenomenon/Baader-Meinhof%20Phenomenon.owl#LearningSolipsism</rdfs:isDefinedBy>
        <rdfs:label xml:lang="en">Learning Solipsism</rdfs:label>
    </owl:NamedIndividual>
    


    <!-- https://raw.githubusercontent.com/ranacoskun/cognitive_bias_ontology/main/Baader-Meinhof%20Phenomenon/Baader-Meinhof%20Phenomenon.owl#RecognisingSolipsism -->

    <owl:NamedIndividual rdf:about="https://raw.githubusercontent.com/ranacoskun/cognitive_bias_ontology/main/Baader-Meinhof%20Phenomenon/Baader-Meinhof%20Phenomenon.owl#RecognisingSolipsism">
        <rdf:type rdf:resource="https://w3id.org/framester/data/framestercore/PerceptionExperience"/>
        <parameter:hasParameter rdf:resource="https://raw.githubusercontent.com/ranacoskun/cognitive_bias_ontology/main/Baader-Meinhof%20Phenomenon/Baader-Meinhof%20Phenomenon.owl#FrequencyOfSolipsism"/>
        <situation:hasSetting rdf:resource="https://raw.githubusercontent.com/ranacoskun/cognitive_bias_ontology/main/Baader-Meinhof%20Phenomenon/Baader-Meinhof%20Phenomenon.owl#Solipsism"/>
        <cbi:influences rdf:resource="https://raw.githubusercontent.com/ranacoskun/cognitive_bias_ontology/main/Baader-Meinhof%20Phenomenon/Baader-Meinhof%20Phenomenon.owl#FrequencyBelief"/>
        <rdfs:comment xml:lang="en">An activity where Jamie encounters the word &quot;solipsism&quot; in a psychology book.</rdfs:comment>
        <rdfs:isDefinedBy>https://raw.githubusercontent.com/ranacoskun/cognitive_bias_ontology/main/Baader-Meinhof%20Phenomenon/Baader-Meinhof%20Phenomenon.owl#RecognisingSolipsism</rdfs:isDefinedBy>
        <rdfs:label xml:lang="en">Recognising Solipsism</rdfs:label>
    </owl:NamedIndividual>
    


    <!-- https://raw.githubusercontent.com/ranacoskun/cognitive_bias_ontology/main/Baader-Meinhof%20Phenomenon/Baader-Meinhof%20Phenomenon.owl#Solipsism -->

    <owl:NamedIndividual rdf:about="https://raw.githubusercontent.com/ranacoskun/cognitive_bias_ontology/main/Baader-Meinhof%20Phenomenon/Baader-Meinhof%20Phenomenon.owl#Solipsism">
        <rdf:type rdf:resource="http://dbpedia.org/ontology/Concept"/>
        <situation:isSettingFor rdf:resource="https://raw.githubusercontent.com/ranacoskun/cognitive_bias_ontology/main/Baader-Meinhof%20Phenomenon/Baader-Meinhof%20Phenomenon.owl#RecognisingSolipsism"/>
        <rdfs:comment xml:lang="en">The term &quot;solipsism&quot; and its meaning that Jamie learns.</rdfs:comment>
        <rdfs:isDefinedBy>https://raw.githubusercontent.com/ranacoskun/cognitive_bias_ontology/main/Baader-Meinhof%20Phenomenon/Baader-Meinhof%20Phenomenon.owl#Solipsism</rdfs:isDefinedBy>
        <rdfs:label xml:lang="en">Solipsism</rdfs:label>
    </owl:NamedIndividual>
    


    <!-- https://raw.githubusercontent.com/ranacoskun/cognitive_bias_ontology/main/Baader-Meinhof%20Phenomenon/Baader-Meinhof%20Phenomenon.owl#SolipsismKnowledge -->

    <owl:NamedIndividual rdf:about="https://raw.githubusercontent.com/ranacoskun/cognitive_bias_ontology/main/Baader-Meinhof%20Phenomenon/Baader-Meinhof%20Phenomenon.owl#SolipsismKnowledge">
        <rdf:type rdf:resource="http://dbpedia.org/ontology/Knowledge"/>
        <reaction:isOutcomeOf rdf:resource="https://raw.githubusercontent.com/ranacoskun/cognitive_bias_ontology/main/Baader-Meinhof%20Phenomenon/Baader-Meinhof%20Phenomenon.owl#LearningSolipsism"/>
        <crm:isAbout rdf:resource="https://raw.githubusercontent.com/ranacoskun/cognitive_bias_ontology/main/Baader-Meinhof%20Phenomenon/Baader-Meinhof%20Phenomenon.owl#Solipsism"/>
        <rdfs:comment xml:lang="en">The knowledge about the philosophical concept of solipsism that Jamie acquires and begins to encounter frequently in various contexts.</rdfs:comment>
        <rdfs:isDefinedBy>https://raw.githubusercontent.com/ranacoskun/cognitive_bias_ontology/main/Baader-Meinhof%20Phenomenon/Baader-Meinhof%20Phenomenon.owl#SolipsismKnowledge</rdfs:isDefinedBy>
        <rdfs:label xml:lang="en">Solipsism Knowledge</rdfs:label>
    </owl:NamedIndividual>
    


    <!-- https://raw.githubusercontent.com/ranacoskun/cognitive_bias_ontology/main/cbi.owl#Jamie -->

    <owl:NamedIndividual rdf:about="https://raw.githubusercontent.com/ranacoskun/cognitive_bias_ontology/main/cbi.owl#Jamie">
        <rdf:type rdf:resource="https://raw.githubusercontent.com/ranacoskun/cognitive_bias_ontology/main/cbi.owl#BiasedAgent"/>
        <exob:isEngagedIn rdf:resource="https://raw.githubusercontent.com/ranacoskun/cognitive_bias_ontology/main/Baader-Meinhof%20Phenomenon/Baader-Meinhof%20Phenomenon.owl#LearningSolipsism"/>
        <exob:isEngagedIn rdf:resource="https://raw.githubusercontent.com/ranacoskun/cognitive_bias_ontology/main/Baader-Meinhof%20Phenomenon/Baader-Meinhof%20Phenomenon.owl#RecognisingSolipsism"/>
        <cbi:affectedBy rdf:resource="https://raw.githubusercontent.com/ranacoskun/cognitive_bias_ontology/main/Baader-Meinhof%20Phenomenon/Baader-Meinhof%20Phenomenon.owl#Baader-MeinhofPhenomenonInstance"/>
        <rdfs:comment xml:lang="en">A biased agent who experiences the Baader-Meinhof phenomenon in our user case.</rdfs:comment>
        <rdfs:isDefinedBy>https://raw.githubusercontent.com/ranacoskun/cognitive_bias_ontology/main/cbi.owl#Jamie</rdfs:isDefinedBy>
        <rdfs:label xml:lang="en">Jamie</rdfs:label>
    </owl:NamedIndividual>
</rdf:RDF>



<!-- Generated by the OWL API (version 4.5.26.2023-07-17T20:34:13Z) https://github.com/owlcs/owlapi -->
